Further work on Fragmenta's proofs

Isabelle/Fragmenta/Fragmenta_SGs.thy
@@ -143,17 +143,11 @@ lemma acyclic_sg_noEI:"EsI SG = {} \<Longrightarrow> acyclicGr (inhG SG)"
   by (simp add: acyclicGr_def inh_noedgesI wf_acyclic inh_def 
       inhG_def emptyG_def relG_def adjacent_def)
 
-definition srcma_ecomp_uni:: "SGr \<Rightarrow> E \<rightharpoonup> MultC"
-  where
-  "srcma_ecomp_uni SG \<equiv> (\<lambda> x. if x \<in> EsTy SG {ecomp duni} then Some (sm (val 1)) else None)"
-
-definition srcma_erel_uni:: "SGr \<Rightarrow> E \<rightharpoonup> MultC"
-  where
-  "srcma_erel_uni SG \<equiv> (\<lambda> x. if x \<in> EsTy SG {erel duni} then Some (sm many) else None)"
-
 definition srcma ::"SGr \<Rightarrow> E \<rightharpoonup> MultC"
 where
-  "srcma SG \<equiv> (srcm SG) ++ srcma_ecomp_uni SG ++ srcma_erel_uni SG"
+  "srcma SG \<equiv> (srcm SG) 
+    ++ (\<lambda> x. if x \<in> EsTy SG {ecomp duni} then Some (sm (val 1)) else None) 
+    ++ (\<lambda> x. if x \<in> EsTy SG {erel duni} then Some (sm many) else None)"
 
 definition multsOk::"SGr \<Rightarrow>bool"
   where
@@ -196,11 +190,11 @@ definition esIncidentst::"SGr \<Rightarrow>V set \<Rightarrow> E set" (infixl "\
 
 lemma esIncidentst_emptySG:
   "emptySG \<circ>\<rightarrow>\<circ>\<^sup>* vs = {}"
-  by (simp add: esIncidentst_def )
+  by (simp add: esIncidentst_def)
 
 lemma esIncidentst_empty_vs:
   "SG \<circ>\<rightarrow>\<circ>\<^sup>* {} = {}"
-  by (simp add: esIncidentst_def )
+  by (simp add: esIncidentst_def)
 
 definition optsVoluntary::"SGr \<Rightarrow>bool"
   where
@@ -209,7 +203,8 @@ definition optsVoluntary::"SGr \<Rightarrow>bool"
 definition inhOk::"SGr \<Rightarrow>bool"
   where
   "inhOk SG \<equiv> (\<forall> v v'. (v, v') \<in> inh SG \<longrightarrow> the (nty SG v) <\<^sub>N\<^sub>T the (nty SG v'))
-    \<and> acyclicGr (inhG SG) \<and> tree (((inhG SG) \<ominus>\<^sub>N\<^sub>S (NsV SG))\<^sup>\<Leftrightarrow>)"
+    \<and> acyclicGr (inhG SG) 
+    \<and> pfun_on (((inhG SG) \<ominus>\<^sub>N\<^sub>S (NsV SG))\<^sup>\<Leftrightarrow>) (Ns SG)(Ns SG)"
 
 definition wf_sg :: "SGr \<Rightarrow> bool"
 where
@@ -219,7 +214,9 @@ where
       \<and> ftotal_on (srcma SG) (EsC SG) MultC_set
       \<and> ftotal_on (tgtm SG) (EsC SG) MultC_set
       \<and> dom (db SG) = EsD SG
-      \<and> multsOk SG"
+      \<and> multsOk SG
+      \<and> optsVoluntary SG
+      \<and> inhOk SG"
 
 lemma wf_sg_wf_g:
   assumes "wf_sg SG"
@@ -271,6 +268,18 @@ lemma NsP_sub_Ns:
   using assms wf_sg_ftotal_on_nty [of SG]
   by (auto simp add: NsP_def NsTy_def ftotal_on_def)
 
+lemma NsO_sub_Ns: 
+  assumes "wf_sg SG"
+  shows "NsO SG \<subseteq> Ns SG"
+  using assms wf_sg_ftotal_on_nty [of SG]
+  by (auto simp add: NsO_def NsTy_def ftotal_on_def)
+
+lemma NsV_sub_Ns: 
+  assumes "wf_sg SG"
+  shows "NsV SG \<subseteq> Ns SG"
+  using assms wf_sg_ftotal_on_nty [of SG]
+  by (auto simp add: NsV_def NsTy_def ftotal_on_def)
+
 lemma wf_g_inhG:
   assumes "wf_g SG"
   shows "wf_g (inhG SG)"
@@ -288,24 +297,29 @@ lemma EsI_sub_Es:
 using assms wf_sg_ftotal_on_ety[of SG]
   by (auto simp add: EsI_def EsTy_sub_Es)
 
-lemma EsC_sub_ES: 
+lemma EsA_sub_Es: 
   assumes "wf_sg SG"
-  shows "EsC SG \<subseteq> Es SG"
+  shows "EsA SG \<subseteq> Es SG"
   using assms wf_sg_ftotal_on_ety[of SG]
-  by (auto simp add: EsC_def EsTy_def ftotal_on_def 
-      EsA_def EsW_def EsD_def)
+  by (auto simp add: EsA_def EsTy_sub_Es)
 
-lemma EsD_sub_ES: 
+lemma EsW_sub_Es: 
+  assumes "wf_sg SG"
+  shows "EsW SG \<subseteq> Es SG"
+  using assms wf_sg_ftotal_on_ety[of SG]
+  by (auto simp add: EsW_def EsTy_sub_Es)
+
+lemma EsD_sub_Es: 
   assumes "wf_sg SG"
   shows "EsD SG \<subseteq> Es SG"
   using assms wf_sg_ftotal_on_ety[of SG]
   by (auto simp add: EsD_def EsTy_def ftotal_on_def)
 
-lemma EsA_sub_ES: 
+lemma EsC_sub_Es: 
   assumes "wf_sg SG"
-  shows "EsA SG \<subseteq> Es SG"
+  shows "EsC SG \<subseteq> Es SG"
   using assms wf_sg_ftotal_on_ety[of SG]
-  by (auto simp add: EsA_def EsTy_def ftotal_on_def)
+  by (auto simp add: EsC_def EsA_sub_Es EsW_sub_Es EsD_sub_Es)
 
 lemma Domain_inh:
   assumes "wf_sg SG"
@@ -316,12 +330,18 @@ lemma Domain_inh:
       restrict_map_def inhG_def intro!: ranI)
 
 lemma Range_inh:
-  assumes h1: "wf_sg SG"
+  assumes "wf_sg SG"
   shows "Range (inh SG) \<subseteq> Ns SG"
   using assms wf_sg_ftotal_on_tgtG[of SG]
   by (auto simp add: inh_def relG_def adjacent_def ftotal_on_def 
       rst_fun_def EsI_def EsTy_def
       restrict_map_def inhG_def intro!: ranI)
+
+lemma inhG_disj_Es:
+  assumes "disjEsGs SG1 SG2"
+  shows "disjEsGs (inhG SG1) (inhG SG2)"
+  using assms EsI_sub_Es
+  by (auto simp add: disjEsGs_def)
 
 lemma inh_sub_inhst: "inh SG \<subseteq>  inhst SG"
   by (auto simp add: inhst_def)
@@ -340,200 +360,29 @@ lemma tgt_restrict_EsA_sub_tgtst:
           tgtr_def
           split: if_splits)
 
+lemma dom_srcst_sub_Es:
+  assumes "wf_sg SG"
+  shows "Domain (srcst SG) \<subseteq> Es SG"
+  using assms EsC_sub_Es
+  by (auto simp add: srcst_def relcomp_unfold dres_def Domain_iff 
+      subsetI)
 
-(*
-lemma in_Es_removeNsNotAdjP_inhG:
-  assumes h1: "is_wf_sg SG" and h2: "e \<in> Es (removeNs (inhG SG) (NsNotAdjP SG))" 
-  shows "\<exists> p. p \<in> NsP SG \<and> (src SG e = Some p \<or> tgt SG e = Some p)"
-  proof -
-    from h1 have h1a: "is_wf_g SG"
-      by (simp add: is_wf_sg_def)
-    from h1a have h1b: "dom (src SG) = Es SG" 
-      by (simp add: is_wf_g_def ftotal_on_def)
-    from h1a have h1c: "dom (tgt SG) = Es SG" 
-      by (simp add: is_wf_g_def ftotal_on_def)
-    from h1a have h1d: "ran (src SG) \<subseteq> Ns SG" 
-      by (simp add: is_wf_g_def ftotal_on_def)
-    from h1a have h1e: "ran (tgt SG) \<subseteq> Ns SG" 
-      by (simp add: is_wf_g_def ftotal_on_def)
-    from h1 have h1f: "is_wf_g (inhG SG)"
-      by (simp add: is_wf_g_inhG)
-    from h1f have h1g: "is_wf_g (removeNs (inhG SG) (NsNotAdjP SG))"
-      using is_wf_remove[where G="inhG SG" and ns="NsNotAdjP SG"]
-      by (simp)
-    from h2 h1g have h2a: "e \<in> dom (src (removeNs (inhG SG) (NsNotAdjP SG)))"
-      by (simp add: is_wf_g_def ftotal_on_def)
-    from h2 h1g have h2b: "e \<in> dom (tgt (removeNs (inhG SG) (NsNotAdjP SG)))"
-      by (simp add: is_wf_g_def ftotal_on_def)
-    from h1b h1c h2 show ?thesis
-    proof (simp add: rst_fun_def restrict_map_def split: if_splits)
-      apply_end(erule conjE, erule conjE, erule conjE, erule conjE)
-      assume h3a: "e \<in> Es SG"
-      from h3a h1b have h3b: "e \<in> dom (src SG)" by simp
-      from h3a h1c have h3c: "e \<in> dom (tgt SG)" by simp
-      assume h3d: "e \<in> EsI SG"
-      assume h3e: "e \<notin> EsId SG" 
-      assume h3f: "src SG e \<notin> Some ` NsNotAdjP SG"
-      hence h3g: "src SG e \<notin> Some ` NsNotAdjP SG \<longrightarrow> src SG e \<in> Some ` NsAdjP SG"
-        using h3b h1d
-        by (simp add: image_def dom_def NsNotAdjP_def)(erule exE, auto intro: ranI)
-      assume h3h: "tgt SG e \<notin> Some ` NsNotAdjP SG"
-      hence h3i: "tgt SG e \<in> Some ` NsAdjP SG"
-        using h3c h1e
-        by (simp add: image_def dom_def NsNotAdjP_def)(erule exE, auto intro: ranI)
-      have h2c: "\<exists>v1 v2. src (removeNs (inhG SG) (NsNotAdjP SG)) e = Some v1
-        \<and> tgt (removeNs (inhG SG) (NsNotAdjP SG)) e = Some v2 \<and> (v1 \<in> NsP SG \<or> v2 \<in> NsP SG)"
-      proof (simp)
-      qed
-        by (auto simp add: rst_fun_def rmv_EsOfNs_def restrict_map_def image_def NsNotAdjP_def 
-          NsAdjP_def dom_def split: if_splits intro!: ranI)
-      from h2a h2b h3a h3d h1d h1e 
-        by (simp add: image_def dom_def NsNotAdjP_def)(erule exE, auto intro: ranI)
-      have h3j: "\<exists> v1 v2 . src SG e \<in> Some ` NsP SG \<or> tgt SG e \<in> Some ` NsP SG"
-        using h3b h3c  
-        proof (simp add: image_def dom_def NsAdjP_def)
-          apply_end(erule exE, erule exE)
-          fix v1 v2
-          assume ha: "src SG e = Some v1"
-          assume hb: "tgt SG e = Some v2"
-          show "(\<exists>x\<in>NsP SG. src SG e = Some x) \<or> (\<exists>x\<in>NsP SG. tgt SG e = Some x)"
-          proof (case_tac "v1 \<in> NsP SG")
-            assume hc: "v1 \<in> NsP SG"
-            from ha hc show "(\<exists>x\<in>NsP SG. src SG e = Some x) \<or> (\<exists>x\<in>NsP SG. tgt SG e = Some x)"
-              by auto
-          next
-            assume hc: "v1 \<notin> NsP SG"
-            show "(\<exists>x\<in>NsP SG. src SG e = Some x) \<or> (\<exists>x\<in>NsP SG. tgt SG e = Some x)"
-            proof (case_tac "v2 \<in> NsP SG")
-              assume hd: "v2 \<in> NsP SG"
-              from hb hd show "(\<exists>x\<in>NsP SG. src SG e = Some x) \<or> (\<exists>x\<in>NsP SG. tgt SG e = Some x)"
-                by auto
-            next
-              assume hd: "v2 \<notin> NsP SG"
-              from hc hd ha hb h3g h3i show "(\<exists>x\<in>NsP SG. src SG e = Some x) \<or> (\<exists>x\<in>NsP SG. tgt SG e = Some x)"
-                by (auto simp add: NsAdjP_def adjacent_def)
-            qed
-          qed
-        qed
-      assume h3h: "tgt SG e \<notin> Some ` NsNotAdjP SG"
-      hence h3i: "\<exists> v. tgt SG e = Some v \<and> v \<in> NsAdjP SG"
-         using h3c h1d by (simp add: image_def dom_def NsNotAdjP_def)
-          (erule exE, auto intro: ranI)
-      show "\<exists>p. p \<in> NsP SG \<and> (src SG e = Some p \<or> tgt SG e = Some p)"
-      proof (rule ccontr)
-        apply_end(simp)
-        assume h4: "\<forall>p. p \<in> NsP SG \<longrightarrow> src SG e \<noteq> Some p \<and> tgt SG e \<noteq> Some p"
-        from h3g show "False"
-        proof
-          apply_end(erule conjE)
-          fix v1
-          assume h5a: "src SG e = Some v1"
-          assume h5b: "v1 \<in> NsAdjP SG"
-          from h5a h5b h1c have h4c: "v1 \<in> NsP SG 
-            \<or> (\<exists>p. p \<in> NsP SG \<and> (adjacent v1 p SG \<or> adjacent p v1 SG))"
-            by (auto simp add: NsNotAdjP_def NsAdjP_def intro: ranI)
-          show "False"
-          proof (case_tac "v1 \<in> NsP SG")
-            assume h6a: "v1 \<in> NsP SG"
-            from h4 h6a have h6b: "src SG e \<noteq> Some v1 \<and> tgt SG e \<noteq> Some v1"
-              by auto
-            from h6b h5a show "False" by auto
-          next
-            assume h6: "v1 \<notin> NsP SG"
-            from h3i show "False"
-            proof
-              apply_end(erule conjE)
-              fix v2
-              assume h7a: "tgt SG e = Some v2"
-              assume h7b: "v2 \<notin> NsNotAdjP SG"
-              from h7a h7b h1d have h7c: "v2 \<in> NsP SG 
-                \<or> (\<exists>p. p \<in> NsP SG \<and> (adjacent v2 p SG \<or> adjacent p v2 SG))"
-                by (auto simp add: NsNotAdjP_def NsAdjP_def intro: ranI)
-                show "False"
-                proof (case_tac "v2 \<in> NsP SG")
-                  assume h8a: "v2 \<in> NsP SG"
-                  from h4 h8a have h8b: "src SG e \<noteq> Some v2 \<and> tgt SG e \<noteq> Some v2"
-                  by auto
-                  from h8b h7a show "False" by auto
-                next
-                  assume h8a: "v2 \<notin> NsP SG"
-                  from h6 h4c have h8b: "(\<exists>p. p \<in> NsP SG 
-                    \<and> (adjacent v1 p SG \<or> adjacent p v1 SG))" by auto
-                  from h8b show "False"
-                  proof
-                    apply_end(erule conjE)
-                    fix p
-                    assume h9a: "p \<in> NsP SG"
-                    from h1 h9a have h9b: "p \<in> Ns SG" 
-                      by (auto simp add: in_NsP_Ns)
-                    assume h9c: "adjacent v1 p SG \<or> adjacent p v1 SG"
-                    from h9a h4 have h9d: "src SG e \<noteq> Some p \<and> tgt SG e \<noteq> Some p"
-                      by auto
-                    from h1 h9b have h9e: "p \<in> NsAdjP SG \<or> p \<in> NsNotAdjP SG" 
-                      by (simp add: in_NsAdjP_or_not)
-                    from h9c h9d h9e show "False" 
-                      by (auto simp add: NsAdjP_def NsNotAdjP_def adjacent_def)
-        from h3i show "\<exists>p. p \<in> NsP SG \<and> src SG e = Some p \<or> tgt SG e = Some p"
-        proof
-          apply_end(erule conjE)
-          fix v2
-          assume h5a: "tgt SG e = Some v2"
-          assume h5b: "v2 \<notin> NsNotAdjP SG"
-          from h5a h5b h1d have h5c: "v2 \<in> NsP SG 
-              \<or> (\<exists>p. p \<in> NsP SG \<and> (adjacent v2 p SG \<or> adjacent p v2 SG))"
-            by (auto simp add: NsNotAdjP_def NsAdjP_def intro: ranI)
-          from h4c show "\<exists>p. p \<in> NsP SG \<and> src SG e = Some p \<or> tgt SG e = Some p"
-          proof 
-            assume h6a: "v1 \<in> NsP SG"
-            then show "\<exists>p. p \<in> NsP SG \<and> src SG e = Some p \<or> tgt SG e = Some p"
-              using h4a by (rule_tac exI[where x="v1"])(auto)
-          next
-            apply_end(erule exE)
-            fix p
-            assume h6a: "p \<in> NsP SG \<and> (adjacent v1 p SG \<or> adjacent p v1 SG)"
-            then show "\<exists>p. p \<in> NsP SG \<and> src SG e = Some p \<or> tgt SG e = Some p"
-            proof (case_tac "p=v1")
-              assume "p=v1"
-              then show "\<exists>p. p \<in> NsP SG \<and> src SG e = Some p \<or> tgt SG e = Some p"
-              using h4a h6a by (rule_tac exI[where x="p"])(auto simp add: adjacent_def)
-            next
-              assume h7a: "p\<noteq>v1"
-              from h5c show "\<exists>p. p \<in> NsP SG \<and> src SG e = Some p \<or> tgt SG e = Some p"
-              proof
-                assume h8a: "v2 \<in> NsP SG"
-                then show "\<exists>p. p \<in> NsP SG \<and> src SG e = Some p \<or> tgt SG e = Some p"
-                using h5a by (rule_tac exI[where x="v2"])(auto)
-              next
-                apply_end(erule exE)
-                fix p2
-                assume h8a: "p2 \<in> NsP SG \<and> (adjacent v2 p2 SG \<or> adjacent p2 v2 SG)"
-                from h6a h8a show "\<exists>p. p \<in> NsP SG \<and> src SG e = Some p \<or> tgt SG e = Some p"
-                proof (case_tac "p=v2")
-                  assume h8b: "p=v2"
-                  from h6a h5a h8b show "\<exists>p. p \<in> NsP SG \<and> src SG e = Some p \<or> tgt SG e = Some p"
-                    by (rule_tac exI[where x="p"])(auto simp add: adjacent_def)
-                next
-                  assume h8b: "p \<noteq> v2"
-                  show "\<exists>p. p \<in> NsP SG \<and> src SG e = Some p \<or> tgt SG e = Some p"
-                  proof (case_tac "p2=v1") 
-                    assume "p2=v1"
-                    then show "\<exists>p. p \<in> NsP SG \<and> src SG e = Some p \<or> tgt SG e = Some p"
-                      using h8a h4a by (rule_tac exI[where x="p2"])(auto simp add: adjacent_def)
-                  next
-                    assume h8b: "p2\<noteq>v1"
-                    show "\<exists>p. p \<in> NsP SG \<and> src SG e = Some p \<or> tgt SG e = Some p"
-                    proof (case_tac "p2=v2")
-                      assume h8c: "p2=v2"
-                      from h6a h5a h8c show "\<exists>p. p \<in> NsP SG \<and> src SG e = Some p \<or> tgt SG e = Some p"
-                        by (rule_tac exI[where x="p2"])(auto simp add: adjacent_def)
-                    next
-                      assume h8c: "p2\<noteq>v2" (*I AM HERE*)
-                      from h6a show "\<exists>p. p \<in> NsP SG \<and> src SG e = Some p \<or> tgt SG e = Some p"
-                      using h4a h6a by (rule_tac exI[where x="p"])(auto simp add: adjacent_def)
-                      by (rule_tac exI[where x="p2"])(auto simp add: adjacent_def)
-          
-  qed*)
-  
+lemma dom_tgtst_sub_Es:
+  assumes "wf_sg SG"
+  shows "Domain (tgtst SG) \<subseteq> Es SG"
+  using assms EsC_sub_Es
+  by (auto simp add: tgtst_def relcomp_unfold dres_def Domain_iff)
+
+lemma esIncidentst_SG_Sub_EsSG:
+  assumes "wf_sg SG"
+  shows "SG \<circ>\<rightarrow>\<circ>\<^sup>* vs \<subseteq> Es SG"
+  using assms dom_srcst_sub_Es[of SG] dom_tgtst_sub_Es[of SG]
+  by (auto simp add: esIncidentst_def)
+
+lemma esIncidentst_Un:
+  shows "SG \<circ>\<rightarrow>\<circ>\<^sup>* (vs1 \<union> vs2) = SG \<circ>\<rightarrow>\<circ>\<^sup>* vs1 \<union> SG \<circ>\<rightarrow>\<circ>\<^sup>* vs2"
+  using esIncidentst_def by auto
+
 
 (*lemma inhG_partitions_disjEsGs:
   shows "disjEsGs (restrict (inhG SG) (Es (inhG SG) - EsP SG)) (restrict (inhG SG) (EsP SG))"
@@ -562,56 +411,6 @@ lemma SG_EsA_no_inh:
   next
   show "{} \<subseteq> EsI SG" by (auto)
   qed
-
-lemma EsR_sub_Es: 
-  assumes h1: "is_wf_sg SG"
-  shows "EsR SG \<subseteq> Es SG"
-  proof -
-    from h1 have h1a: "ftotal_on (ety SG) (Es SG) SGETy_set"
-      by (simp add: is_wf_sg_def)
-    from h1a show ?thesis
-      by (auto simp add: EsR_def EsTy_def ftotal_on_def)
-  qed
-
-lemma in_EsR_in_Es:
-  assumes h1: "is_wf_sg SG" and h2: "x \<in> EsR SG"
-  shows "x \<in> (Es SG)"
-  proof -
-    from assms show ?thesis
-    using EsR_sub_Es[where SG="SG"]
-    by (auto) 
-  qed
-
-lemma EsRP_sub_Es: 
-  assumes h1: "is_wf_sg SG"
-  shows "EsRP SG \<subseteq> Es SG"
-  proof -
-    from h1 have h1a: "ftotal_on (ety SG) (Es SG) SGETy_set"
-      by (simp add: is_wf_sg_def)
-    from h1a show ?thesis
-      by (auto simp add: EsRP_def EsR_def EsTy_def ftotal_on_def)
-  qed
-
-lemma in_EsRP_in_Es:
-  assumes h1: "is_wf_sg SG" and h2: "e \<in> EsRP SG"
-  shows "e \<in> Es SG"
-  proof -
-    from assms show ?thesis
-    using EsRP_sub_Es[where SG="SG"]
-    by (auto) 
-  qed
-
-lemma in_EsRP_src_proxy:
-  assumes h1: "e \<in> EsRP SG"
-  shows "\<exists> v. (src SG) e = Some v \<and> v \<in> (NsP SG)"
-  using assms by (auto simp add: EsRP_def)
-
-(*lemma SG_in_EsA:
-  assumes "(ety SG) e = Some erelbi"
-  shows "e \<in> EsA SG"
-proof -
-  from assms show ?thesis by (simp add: EsA_def EsTy_def)
-qed*)
 
 
 lemma inhst_inh_subsetid: "r \<subseteq> Id \<Longrightarrow> inhst SG = (inh SG-r)^*"
@@ -698,11 +497,6 @@ lemma the_tgt_in_tgtst:
   qed
 *)
 
-(*The following lemmas shows that the source or target of an edge is also in the extended set if the edge is of type 
-association. In short: 
-+ If it is in src, it is in src*
-+ If it is in tgt, it is in tgt*)
-
  
 (*lemma "\<lbrakk>is_wf_sg SG; e \<in> EsA(SG)\<rbrakk> \<Longrightarrow> \<exists> v. tgt SG e = Some v \<and> (e, v) \<in> tgtst SG"
   apply (frule tgt_aedge_sg, simp)
@@ -767,7 +561,7 @@ next
       hence h: "x \<in> Es SG1 \<and> x \<in> Es SG2" 
         using assms wf_sg_ftotal_on_srcma[of SG1] 
         wf_sg_ftotal_on_srcma[of SG2] 
-         EsC_sub_ES[of SG1] EsC_sub_ES[of SG2] 
+         EsC_sub_Es[of SG1] EsC_sub_Es[of SG2] 
          srcm_sub_srcma[of SG1] srcm_sub_srcma[of SG2]
          disjGs_imp_disjEsGs[of SG1 SG2]
         by (auto simp add: disjEsGs_def ftotal_on_def)
@@ -783,22 +577,31 @@ next
     using assms wf_sg_ftotal_on_tgtm[of SG1]
       wf_sg_ftotal_on_tgtm[of SG2]
       map_add_comm[of "tgtm SG1" "tgtm SG2"] 
-      EsC_sub_ES[of SG1] EsC_sub_ES[of SG2]
+      EsC_sub_Es[of SG1] EsC_sub_Es[of SG2]
       disjGs_imp_disjEsGs[of SG1 SG2]
     by (auto simp add: disjEsGs_def ftotal_on_def)
 next
   show "db SG1 ++ db SG2 = db SG2 ++ db SG1"
     using assms wf_sg_dom_db[of SG1] wf_sg_dom_db[of SG2]
-      EsD_sub_ES[of SG1] EsD_sub_ES[of SG2]
+      EsD_sub_Es[of SG1] EsD_sub_Es[of SG2]
       map_add_comm[of "db SG1" "db SG2"] 
       disjGs_imp_disjEsGs[of SG1 SG2]
     by (auto simp add: disjEsGs_def)(force)
 qed
-    
+
+lemma Ns_cupSG[simp]: "Ns (SG1 USG SG2) = (Ns SG1) \<union> (Ns SG2)"
+  by (simp add: cupSG_def)
+
 lemma src_cupSG[simp]: "src (SG1 USG SG2) = src SG1 ++ src SG2"
   by (simp add: cupSG_def)
 
 lemma tgt_cupSG[simp]: "tgt (SG1 USG SG2) = tgt SG1 ++ tgt SG2"
+  by (simp add: cupSG_def)
+
+lemma ety_cupSG[simp]: "ety (SG1 USG SG2) = ety SG1 ++ ety SG2"
+  by (simp add: cupSG_def)
+
+lemma nty_cupSG[simp]: "nty (SG1 USG SG2) = nty SG1 ++ nty SG2"
   by (simp add: cupSG_def)
 
 lemma srcm_cupSG[simp]: "srcm (SG1 USG SG2) = srcm SG1 ++ srcm SG2"
@@ -902,143 +705,610 @@ lemma EsC_USG:
   shows "EsR (SG1 USG SG2) = (EsR SG1 \<union> EsR SG2)"
   using h1 h2 h3 by (simp add: EsR_def EsTy_USG) *)
 
-lemma NsP_disj_dist: 
+lemma NsP_USG: 
   assumes "wf_sg SG1" and "wf_sg SG2" and "disjGs SG1 SG2"
   shows "NsP (SG1 USG SG2) = NsP SG1 \<union> NsP SG2"
   using assms by (simp add: NsP_def NsTy_USG)
- 
-(*lemma EsRP_Un_EsR_1: "\<lbrakk>disjGs SG1 SG2; is_wf_sg SG1; is_wf_sg SG2; 
-  x \<in> EsR SG1; x \<in> EsRP SG1 \<or> x \<in> EsRP SG2\<rbrakk>
-  \<Longrightarrow>x \<in> EsRP SG1"
-  proof -
-    assume h1: "disjGs SG1 SG2"
-    have h1a: "Es SG1 \<inter> Es SG2 = {}"
-      using h1 by (simp add: disjGs_def disjEsGs_def)
-    assume h2: "is_wf_sg SG1"
-    from h2 have h2a: "ftotal_on (ety SG1) (Es SG1) SGETy_set"
-      by (simp add: is_wf_sg_def)
-    assume h3: "is_wf_sg SG2"
-    from h3 have h3a: "ftotal_on (ety SG2) (Es SG2) SGETy_set"
-      by (simp add: is_wf_sg_def)
-    assume h4: "x \<in> EsR SG1"
-    from h4 have h4a: "x \<in> Es SG1"
-      using h2a by (auto simp add: EsR_def EsTy_def ftotal_on_def)
-    from h4 have h4b: "x \<notin> Es SG2" 
-      using h3a h1a h2a by (auto simp add: EsR_def EsTy_def ftotal_on_def)
-    from h4 have h4c: "x \<notin> EsR SG2" 
-      using h3a h1a h4b by (auto simp add: EsR_def EsTy_def ftotal_on_def)
-    assume h4: "x \<in> EsRP SG1 \<or> x \<in> EsRP SG2"
-    show ?thesis
-    using h1a h3 h3a h4 h4c by (simp add: EsRP_def)
-  qed
 
-lemma EsRP_disj_dist: "\<lbrakk>is_wf_sg SG1; is_wf_sg SG2; disjGs SG1 SG2\<rbrakk>
-  \<Longrightarrow>EsRP (SG1 USG SG2) = EsRP SG1 \<union> EsRP SG2"
-proof -
-    assume h1: "disjGs SG1 SG2"
-    have h1a: "Es SG1 \<inter> Es SG2 = {}"
-      using h1 by (simp add: disjGs_def disjEsGs_def)
-    have h1b: "Ns SG1 \<inter> Ns SG2 = {}"
-      using h1 by (simp add: disjGs_def)
-    assume h2: "is_wf_sg SG1"
-    have h2a: "ftotal_on (ety SG1) (Es SG1) SGETy_set"
-      using h2 by (simp add: is_wf_sg_def)
-    have h2b: "ftotal_on (src SG1) (Es SG1) (Ns SG1)"
-      using h2 by (simp add: is_wf_sg_def is_wf_g_def)
-    from h2b have h2c: "dom (src SG1) = Es SG1"
-      by (simp add: ftotal_on_def)
-    from h2b have h2d: "ran (src SG1) \<subseteq> Ns SG1"
-      by (simp add: ftotal_on_def)
-    have "ftotal_on (nty SG1) (Ns SG1) SGNTy_set"
-      using h2 by (simp add: is_wf_sg_def)
-    then have h2e: "dom (nty SG1) = Ns SG1"
-      by (simp add: ftotal_on_def)
-    assume h3: "is_wf_sg SG2"
-    have h3a: "ftotal_on (ety SG2) (Es SG2) SGETy_set"
-      using h3 by (simp add: is_wf_sg_def)
-    have h3b: "ftotal_on (src SG2) (Es SG2) (Ns SG2)"
-      using h3 by (simp add: is_wf_sg_def is_wf_g_def)
-    from h3b have h3c: "dom (src SG2) = Es SG2"
-      by (simp add: ftotal_on_def)
-    from h3b have h3d: "ran (src SG2) \<subseteq> Ns SG2"
-      by (simp add: ftotal_on_def)
-    have h4: "dom (ety SG1) \<inter> dom (ety SG2) = {}" 
-      using h1a h2a h3a by (simp add: ftotal_on_dom)
-    have h5: "dom (src SG1) \<inter> dom (src SG2) = {}"
-      using h1a h2c h3c by simp
-    from h4 have h6: "EsR SG1 \<inter> EsR SG2 = {}" 
-      by (auto simp add: EsR_def EsTy_def vimage_def)
-    show "EsRP (SG1 USG SG2) = EsRP SG1 \<union> EsRP SG2"
+lemma NsO_USG: 
+  assumes "wf_sg SG1" and "wf_sg SG2" and "disjGs SG1 SG2"
+  shows "NsO (SG1 USG SG2) = NsO SG1 \<union> NsO SG2"
+  using assms by (simp add: NsO_def NsTy_USG)
+
+lemma NsV_USG: 
+  assumes "wf_sg SG1" and "wf_sg SG2" and "disjGs SG1 SG2"
+  shows "NsV (SG1 USG SG2) = NsV SG1 \<union> NsV SG2"
+  using assms by (simp add: NsV_def NsTy_USG)
+
+lemma dom_srcr_eq_Es:
+  assumes "wf_sg SG" 
+  shows "Domain (srcr SG) = Es SG"
+  using assms wf_sg_wf_g[of SG] dom_src_G[of SG] dom_tgt_G[of SG]
+  by (auto simp add: srcr_def pfunToRel_def dres_def EsW_sub_Es)
+
+lemma dom_tgtr_eq_Es:
+  assumes "wf_sg SG" 
+  shows "Domain (tgtr SG) = Es SG"
+  using assms wf_sg_wf_g[of SG] dom_src_G[of SG] dom_tgt_G[of SG]
+  by (auto simp add: tgtr_def pfunToRel_def dres_def EsW_sub_Es)
+
+lemma ran_srcr_sub_Ns:
+  assumes "wf_sg SG" 
+  shows "Range (srcr SG) \<subseteq> Ns SG"
+  using assms wf_sg_wf_g[of SG] ran_src_G[of SG] ran_tgt_G[of SG]
+  by (auto simp add: srcr_def pfunToRel_def dres_def EsW_sub_Es 
+      ran_def Range_iff)
+
+lemma ran_tgtr_sub_Ns:
+  assumes "wf_sg SG" 
+  shows "Range (tgtr SG) \<subseteq> Ns SG"
+  using assms wf_sg_wf_g[of SG] ran_src_G[of SG] ran_tgt_G[of SG]
+  by (auto simp add: tgtr_def pfunToRel_def dres_def EsW_sub_Es 
+      ran_def Range_iff)
+
+lemma esIncidentst_disjoint_vs:
+  assumes "wf_sg SG" and "vs \<inter> Ns SG = {}"
+  shows "SG \<circ>\<rightarrow>\<circ>\<^sup>* vs = {}"
+proof (rule ccontr)
+  assume "SG \<circ>\<rightarrow>\<circ>\<^sup>* vs \<noteq> {}"
+  hence "\<exists> e v. v \<in> vs \<and> ((e, v) \<in> (srcst SG) \<or> (e, v) \<in> (tgtst SG))" 
+    by (auto simp add: esIncidentst_def)
+  then show "False"
+  proof (clarsimp)
+    fix e v
+    assume h1:"v \<in> vs" 
+    assume "(e, v) \<in> (srcst SG) \<or> (e, v) \<in> (tgtst SG)"
+    then show "False"
     proof
-      show "EsRP (SG1 USG SG2) \<subseteq> EsRP SG1 \<union> EsRP SG2"
-        proof
-          fix x 
-          assume h7: "x \<in> EsRP (SG1 USG SG2)"
-          then have h7a: "x \<in> EsR SG1 \<or> x \<in> EsR SG2"
-            using h1 h2 h3 by (simp add: EsRP_def EsR_disj_dist)
-          from h7 show "x \<in> EsRP SG1 \<union> EsRP SG2"
-            proof (case_tac "x \<in> EsR SG1")
-              assume h8: "x \<in> EsR SG1"
-              have h8a: "\<exists> v. src SG1 x = Some v \<and> v \<in> Ns SG1"
-                using h8 h2 h2c h2d domD[where m="src SG1" and a ="x"]
-                  ranI[where m="src SG1" and a ="x"]
-                by (simp add: in_EsR_in_Es)(erule exE, auto)
-              from h8 have h8c: "x \<in> EsRP SG1" 
-                using h1 h2 h3 h7 h4 h5 h8a h2c h2d h1b
-                by (simp add: EsRP_def EsR_disj_dist map_add_app_disj NsP_disj_dist in_EsR_in_Es)
-                  (erule exE, auto simp add: in_NsP_Ns)
-              from h8c show "x \<in> EsRP SG1 \<union> EsRP SG2"
-                using h8 by (simp)
-            next
-              assume h8: "x \<notin> EsR SG1"
-              show "x \<in> EsRP SG1 \<union> EsRP SG2"
-              proof (case_tac "x \<in> EsR SG2")
-                assume h9: "x \<in> EsR SG2"
-              have h9a: "\<exists> v. src SG2 x = Some v \<and> v \<in> Ns SG2 \<and> v \<notin> Ns SG1"
-                using h9 h3 h1b h3c h3d domD[where m="src SG2" and a ="x"]
-                  ranI[where m="src SG2" and a ="x"]
-                  EsR_sub_Es[where SG="SG2"]
-                by (simp add: in_EsR_in_Es)(erule exE, auto)
-              from h9 have h9c: "x \<in> EsRP SG2" 
-                using h1 h2 h3 h7 h4 h5 h8 h9a h2c h3c h3d
-                by (auto simp add: EsRP_def EsR_disj_dist map_add_app_disj NsP_disj_dist 
-                  in_EsR_in_Es in_NsP_Ns split: if_splits)
-              from h9c show "x \<in> EsRP SG1 \<union> EsRP SG2"
-                by simp
-            next
-              assume h9: "x \<notin> EsR SG2"
-              from h8 h9 show "x \<in> EsRP SG1 \<union> EsRP SG2"
-                using h7a by simp
-            qed
+      assume "(e, v) \<in> srcst SG"
+      hence "\<exists> v'. (e, v') \<in> srcr SG \<and> (v, v') \<in> (inhst SG)" 
+        by (auto simp add: srcst_def dres_def relcomp_unfold)
+      then show "False"
+      proof
+        fix v' 
+        assume h:"(e, v') \<in> srcr SG \<and> (v, v') \<in> inhst SG"
+        then show "False"
+        proof (case_tac "v = v'")
+          assume "v = v'"
+          hence "v \<in> Ns SG"
+            using h ran_srcr_sub_Ns[of SG] assms(1)
+            by (auto simp add: Range_iff)
+          then show "False"
+            using assms h1 by auto
+        next
+          assume h': "v \<noteq> v'"
+          have "(v, v') \<in> inhst SG" using h by auto
+          hence "v \<in> Domain (inh SG)" 
+            using h' 
+            by (simp add: inhst_def in_rtrcl_in_Domain_if_neq)
+          then show "False"
+            using assms Domain_inh h1 by auto
         qed
       qed
-   next
-      show "EsRP SG1 \<union> EsRP SG2 \<subseteq> EsRP (SG1 USG SG2)"
-        proof
-          fix x
-          assume h7: "x \<in> EsRP SG1 \<union> EsRP SG2"
-          from h7 have h7a: "x \<in> EsRP SG1 \<or> x \<in> EsRP SG2" 
-            by simp
-          show "x \<in> EsRP (SG1 USG SG2)"
-          proof (case_tac "x \<in> EsRP SG1")
-            assume h8: "x \<in> EsRP SG1"
-            from h8 show "x \<in> EsRP (SG1 USG SG2)"
-              using h1 h2 h3 h5 h2c
-              by (auto simp add: EsRP_def EsR_disj_dist NsP_disj_dist map_add_app_disj
-                in_EsR_in_Es)
-          next
-            assume h8: "x \<notin> EsRP SG1"
-            from h8 h7a have h8a: "x \<in> EsRP SG2"
-              by simp
-            from h8a show "x \<in> EsRP (SG1 USG SG2)"
-              using h1 h2 h3 h5 h2c
-              by (auto simp add: EsRP_def EsR_disj_dist NsP_disj_dist map_add_app_disj
-                in_EsR_in_Es)
-          qed
+    next
+      assume "(e, v) \<in> tgtst SG"
+      hence "\<exists> v'. (e, v') \<in> tgtr SG \<and> (v, v') \<in> (inhst SG)" 
+        by (auto simp add: tgtst_def dres_def relcomp_unfold)
+      then show "False"
+      proof
+        fix v' 
+        assume h:"(e, v') \<in> tgtr SG \<and> (v, v') \<in> inhst SG"
+        then show "False"
+        proof (case_tac "v = v'")
+          assume "v = v'"
+          hence "v \<in> Ns SG"
+            using h ran_tgtr_sub_Ns[of SG] assms(1)
+            by (auto simp add: Range_iff)
+          then show "False"
+            using assms h1 by auto
+        next
+          assume h': "v \<noteq> v'"
+          have "(v, v') \<in> inhst SG" using h by auto
+          hence "v \<in> Domain (inh SG)" 
+            using h' 
+            by (simp add: inhst_def in_rtrcl_in_Domain_if_neq)
+          then show "False"
+            using assms Domain_inh h1 by auto
         qed
-   qed
-qed *)
+      qed
+    qed
+  qed
+qed
 
+lemma srcr_USG: 
+  assumes "wf_sg SG1" and "wf_sg SG2" and "disjGs SG1 SG2"
+  shows "srcr (SG1 USG SG2) = srcr SG1 \<union> srcr SG2"  
+proof -
+  have h1: "EsW SG2 \<inter> Domain (pfunToRel (tgt SG1)) = {}"
+    using assms EsW_sub_Es[of SG2] wf_sg_wf_g[of SG1]
+      wf_sg_wf_g[of SG2]
+      disjGs_imp_disjEsGs[of SG1 SG2] 
+      dom_tgt_G[of SG1] dom_tgt_G[of SG2]
+    by (auto simp add: disjEsGs_def pfunToRel_iff)(force)
+  have h2: "EsW SG1 \<inter> Domain (pfunToRel (tgt SG2)) = {}"
+    using assms EsW_sub_Es[of SG1] wf_sg_wf_g[of SG1]
+      wf_sg_wf_g[of SG2]
+      disjGs_imp_disjEsGs[of SG1 SG2] 
+      dom_tgt_G[of SG1] dom_tgt_G[of SG2]
+    by (auto simp add: disjEsGs_def pfunToRel_iff)(force)
+  show ?thesis
+  using assms disjGs_imp_disjEsGs[of SG1 SG2] 
+    wf_sg_wf_g[of SG1] wf_sg_wf_g[of SG2]
+    dom_src_G[of SG1] dom_src_G[of SG2]
+    dom_tgt_G[of SG1] dom_tgt_G[of SG2]
+    EsW_sub_Es[of SG1] EsW_sub_Es[of SG2]
+  by (auto simp add: srcr_def pfunToRel_map_add disjEsGs_def h1 h2
+      dres_union_r EsW_USG dres_union_set dres_not_in_dom)
+qed
+
+lemma tgtr_USG: 
+  assumes "wf_sg SG1" and "wf_sg SG2" and "disjGs SG1 SG2"
+  shows "tgtr (SG1 USG SG2) = tgtr SG1 \<union> tgtr SG2"  
+proof -
+  have h1: "EsW SG2 \<inter> Domain (pfunToRel (src SG1)) = {}"
+    using assms EsW_sub_Es[of SG2] wf_sg_wf_g[of SG1]
+      wf_sg_wf_g[of SG2]
+      disjGs_imp_disjEsGs[of SG1 SG2] 
+      dom_src_G[of SG1] dom_src_G[of SG2]
+    by (auto simp add: disjEsGs_def pfunToRel_iff)(force)
+  have h2: "EsW SG1 \<inter> Domain (pfunToRel (src SG2)) = {}"
+    using assms EsW_sub_Es[of SG1] wf_sg_wf_g[of SG1]
+      wf_sg_wf_g[of SG2]
+      disjGs_imp_disjEsGs[of SG1 SG2] 
+      dom_src_G[of SG1] dom_src_G[of SG2]
+    by (auto simp add: disjEsGs_def pfunToRel_iff)(force)
+  show ?thesis
+  using assms disjGs_imp_disjEsGs[of SG1 SG2] 
+    wf_sg_wf_g[of SG1] wf_sg_wf_g[of SG2]
+    dom_src_G[of SG1] dom_src_G[of SG2]
+    dom_tgt_G[of SG1] dom_tgt_G[of SG2]
+    EsW_sub_Es[of SG1] EsW_sub_Es[of SG2]
+  by (auto simp add: tgtr_def pfunToRel_map_add disjEsGs_def h1 h2
+      dres_union_r EsW_USG dres_union_set dres_not_in_dom)
+qed
+
+lemma restrict_cup_wf_1: 
+  assumes "wf_sg SG1" and "wf_sg SG2" and "disjGs SG1 SG2"
+  shows "SG1 \<bowtie>\<^sub>E\<^sub>S (EsI SG1 \<union> EsI SG2) = SG1 \<bowtie>\<^sub>E\<^sub>S EsI SG1"
+proof -
+  have "EsI SG2 \<inter> Es SG1 = {}"
+    using assms(2) assms(3) EsI_sub_Es[of SG2]
+    by (auto simp add: disjGs_def disjEsGs_def)
+  then show ?thesis
+    using assms wf_sg_wf_g[of SG1] wf_sg_wf_g[of SG2]
+    by (simp add: restrict_dist_cup_es)
+qed
+
+lemma disjGs_inhG:
+  assumes "wf_sg SG1" and "wf_sg SG2" and "disjGs SG1 SG2"
+  shows "disjGs (inhG SG1) (inhG SG2)"
+proof (simp add: disjGs_def)
+  apply_end(rule conjI)
+  show "rst_Ns SG1 (EsI SG1) \<inter> rst_Ns SG2 (EsI SG2) = {}"
+    using assms wf_sg_wf_g[of SG1] wf_sg_wf_g[of SG2]
+      ran_src_G[of SG1] ran_src_G[of SG2] 
+      ran_tgt_G[of SG1] ran_tgt_G[of SG2] 
+      ran_restrict_sub[of "src SG1" "EsI SG1"]
+      ran_restrict_sub[of "src SG2" "EsI SG2"]
+      ran_restrict_sub[of "tgt SG1" "EsI SG1"]
+      ran_restrict_sub[of "tgt SG2" "EsI SG2"]
+    unfolding rst_Ns_def disjGs_def by force
+next
+  apply_end(rule conjI)
+  show "rst_Ns SG1 (EsI SG1) \<inter> (Es SG1 \<inter> EsI SG1) = {}"
+    using assms(1) assms(3) disj_V_E wf_sg_wf_g[of SG1]
+      ran_restrict_sub[of "src SG1" "EsI SG1"]
+      ran_restrict_sub[of "tgt SG1" "EsI SG1"]
+    by (auto simp add: rst_Ns_def wf_g_def disjGs_def 
+        ftotal_on_def)
+next
+  apply_end(rule conjI)
+  show "rst_Ns SG1 (EsI SG1) \<inter> (Es SG2 \<inter> EsI SG2) = {}"
+    using assms(1) assms(3) disj_V_E wf_sg_wf_g[of SG1]
+      ran_restrict_sub[of "src SG1" "EsI SG1"]
+      ran_restrict_sub[of "tgt SG1" "EsI SG1"]
+    by (auto simp add: rst_Ns_def wf_g_def disjGs_def 
+        ftotal_on_def)
+next
+  apply_end(rule conjI)
+  show "rst_Ns SG2 (EsI SG2) \<inter> (Es SG1 \<inter> EsI SG1) = {}"
+    using assms(2) assms(3) disj_V_E wf_sg_wf_g[of SG2]
+      ran_restrict_sub[of "src SG2" "EsI SG2"]
+      ran_restrict_sub[of "tgt SG2" "EsI SG2"]
+    by (auto simp add: rst_Ns_def wf_g_def disjGs_def 
+        ftotal_on_def)
+next
+  apply_end(rule conjI)
+  show "rst_Ns SG2 (EsI SG2) \<inter> (Es SG2 \<inter> EsI SG2) = {}"
+    using assms(2) assms(3) disj_V_E wf_sg_wf_g[of SG2]
+      ran_restrict_sub[of "src SG2" "EsI SG2"]
+      ran_restrict_sub[of "tgt SG2" "EsI SG2"]
+    by (auto simp add: rst_Ns_def wf_g_def disjGs_def 
+        ftotal_on_def)
+next
+  show "Es SG1 \<inter> EsI SG1 \<inter> (Es SG2 \<inter> EsI SG2) = {}"
+    using assms EsI_sub_Es[of SG1] EsI_sub_Es[of SG2]
+    disjGs_imp_disjEsGs[of SG1 SG2]
+    by (auto simp add:  disjEsGs_def)
+qed
+
+lemma inhG_USG:
+  assumes "wf_sg SG1" and "wf_sg SG2" and "disjGs SG1 SG2"
+  shows "inhG (SG1 USG SG2) = inhG (SG1) UG  inhG (SG2)"
+proof -
+  have h: "EsI SG1 \<union> EsI SG2 = EsI SG2 \<union> EsI SG1" by auto
+  show ?thesis
+  using assms disjGs_imp_disjEsGs[of SG1 SG2]
+    restrict_cup_wf_1[of SG2 SG1] restrict_cup_wf_1[of SG1 SG2]
+  by (simp add: inhG_def restrict_USG EsI_USG 
+      disjGs_sym h)
+qed
+
+lemma inh_USG:
+  assumes "wf_sg SG1" and "wf_sg SG2" and "disjGs SG1 SG2"
+  shows "inh (SG1 USG SG2) = inh (SG1) \<union>  inh (SG2)"
+proof -
+  have h1: "EsI SG1 \<union> EsI SG2 = EsI SG2 \<union> EsI SG1" by auto
+  have h2: "SG1 \<bowtie>\<^sub>E\<^sub>S EsI SG1 = inhG SG1" 
+    by (simp add: inhG_def)
+  have h3: "SG2 \<bowtie>\<^sub>E\<^sub>S EsI SG2 = inhG SG2" 
+    by (simp add: inhG_def)
+  show ?thesis
+  using assms disjGs_imp_disjEsGs[of SG1 SG2]
+      wf_sg_wf_g[of SG1] wf_sg_wf_g[of SG2]
+      disjGs_inhG[of SG1 SG2] wf_g_inhG[of SG1] wf_g_inhG[of SG2]
+      disjGs_imp_disjEsGs[of "inhG SG1" "inhG SG2"]
+      restrict_cup_wf_1[of SG2 SG1] restrict_cup_wf_1[of SG1 SG2]
+  by (simp add: inh_def inhG_def restrict_USG EsI_USG 
+      disjGs_sym h1, (subst h2)+, (subst h3)+)
+      (simp add: relG_UG)
+qed
+
+lemma inh_disj_SGs_disj_fields: 
+  assumes "wf_sg SG1" and "wf_sg SG2" and h3: "disjGs SG1 SG2"
+  shows "Field (inh SG1) \<inter> Field (inh SG2) = {}"
+  using assms disjGs_inhG[of SG1 SG2] wf_sg_wf_g[of SG1]
+        wf_sg_wf_g[of SG2] wf_g_inhG[of SG1] wf_g_inhG[of SG2] 
+        by (simp add: inh_def relG_disj_Gs)
+
+lemma inhst_USG: 
+  assumes "wf_sg SG1" and "wf_sg SG2" and "disjGs SG1 SG2"
+  shows "inhst (SG1 USG SG2) = inhst SG1 \<union> inhst SG2"
+  using assms
+      by (simp add: inhst_def inh_USG 
+          inh_disj_SGs_disj_fields rtrancl_disj_dist_Un)
+
+lemma srcst_USG: 
+  assumes "wf_sg SG1" and "wf_sg SG2" and "disjGs SG1 SG2"
+  shows "srcst (SG1 USG SG2) = srcst SG1 \<union> srcst SG2"
+proof
+  show "srcst (SG1 USG SG2) \<subseteq> srcst SG1 \<union> srcst SG2"
+  proof (rule subrelI)
+    fix e v 
+    assume "(e, v) \<in> srcst (SG1 USG SG2)"
+    hence "\<exists> v'. (e, v') \<in>  EsC (SG1 USG SG2) \<lhd>srcr (SG1 USG SG2) 
+      \<and> (v, v') \<in> inhst (SG1 USG SG2)" 
+      using assms by (auto simp add: srcst_def)
+    then show "(e, v) \<in> srcst SG1 \<union> srcst SG2"
+    proof 
+      fix v'
+      assume h: "(e, v') \<in> EsC (SG1 USG SG2) \<lhd> srcr (SG1 USG SG2) \<and>
+         (v, v') \<in> inhst (SG1 USG SG2)"
+      hence "e \<in> EsC SG1 \<or> e \<in> EsC SG2"
+        using assms by (simp add: EsC_USG dres_def)
+      then show "(e, v) \<in> srcst SG1 \<union> srcst SG2"
+      proof
+        assume "e \<in> EsC SG1"
+        hence "e \<in> Es SG1" using assms EsC_sub_Es[of SG1] by auto
+        hence "(e, v') \<in> srcr SG1"
+          using assms h EsC_sub_Es[of SG1] 
+          disjGs_imp_disjEsGs[of SG1 SG2]
+          dom_srcr_eq_Es[of SG1] dom_srcr_eq_Es[of SG2]
+          by (auto simp add: srcr_USG EsC_USG dres_def disjEsGs_def)
+        hence "v' \<in> Ns SG1" 
+          using assms ran_srcr_sub_Ns[of SG1] by (auto)
+        have "(v, v') \<in> inhst SG1"
+        proof (rule ccontr)
+          assume "(v, v') \<notin>  inhst SG1"
+          then show "False"
+          proof (case_tac "v = v'")
+            assume "v = v'"
+            then show "False" 
+              using \<open>(v, v') \<notin>  inhst SG1\<close>
+            by (auto simp add: inhst_def)
+          next
+            assume "v \<noteq> v'"
+            hence "(v, v') \<in> inhst SG2"
+              using \<open>(v, v') \<notin>  inhst SG1\<close> h assms
+              by (auto simp add: inhst_USG EsC_USG srcr_USG )
+            hence "v' \<in> Range(inh SG2)" 
+              using \<open>v \<noteq> v'\<close>
+              by (simp add: in_trancl_in_Range inhst_def 
+                  rtrancl_eq_or_trancl)
+              then show "False"
+                using assms \<open>v' \<in> Ns SG1\<close> Range_inh[of SG2]
+                by (auto simp add: inhst_def disjGs_def)
+          qed
+        qed 
+        hence "(e, v) \<in> srcst SG1"
+          using \<open>e \<in> EsC SG1\<close> \<open>(e, v') \<in> srcr SG1\<close> 
+          by (auto simp add: srcst_def dres_def)
+        then show "(e, v) \<in> srcst SG1 \<union> srcst SG2" 
+           by simp
+      next
+        assume "e \<in> EsC SG2"
+        hence "e \<in> Es SG2" using assms EsC_sub_Es[of SG2] by auto
+        hence "(e, v') \<in> srcr SG2"
+          using assms h EsC_sub_Es[of SG2] 
+          disjGs_imp_disjEsGs[of SG1 SG2]
+          dom_srcr_eq_Es[of SG1] dom_srcr_eq_Es[of SG2]
+          by (auto simp add: srcr_USG EsC_USG dres_def disjEsGs_def)
+        hence "v' \<in> Ns SG2" 
+          using assms ran_srcr_sub_Ns[of SG2] by (auto)
+        have "(v, v') \<in> inhst SG2"
+        proof (rule ccontr)
+          assume "(v, v') \<notin>  inhst SG2"
+          then show "False"
+          proof (case_tac "v = v'")
+            assume "v = v'"
+            then show "False" 
+              using \<open>(v, v') \<notin>  inhst SG2\<close>
+            by (auto simp add: inhst_def)
+          next
+            assume "v \<noteq> v'"
+            hence "(v, v') \<in> inhst SG1"
+              using \<open>(v, v') \<notin>  inhst SG2\<close> h assms
+              by (auto simp add: inhst_USG EsC_USG srcr_USG )
+            hence "v' \<in> Range(inh SG1)" 
+              using \<open>v \<noteq> v'\<close>
+              by (simp add: in_trancl_in_Range inhst_def 
+                  rtrancl_eq_or_trancl)
+            then show "False"
+              using assms \<open>v' \<in> Ns SG2\<close> Range_inh[of SG1]
+              by (auto simp add: inhst_def disjGs_def)
+          qed
+        qed 
+        hence "(e, v) \<in> srcst SG2"
+          using \<open>e \<in> EsC SG2\<close> \<open>(e, v') \<in> srcr SG2\<close> 
+          by (auto simp add: srcst_def dres_def)
+        then show "(e, v) \<in> srcst SG1 \<union> srcst SG2" 
+          by simp
+      qed
+    qed
+  qed
+next
+  show "srcst SG1 \<union> srcst SG2 \<subseteq> srcst (SG1 USG SG2)"
+  proof (rule subrelI)
+    fix e v
+    assume "(e, v) \<in> srcst SG1 \<union> srcst SG2"
+    then show "(e, v) \<in> srcst (SG1 USG SG2)"
+    proof
+      assume "(e, v) \<in> srcst SG1"
+      hence "\<exists> v'. (e, v') \<in> EsC SG1 \<lhd> srcr SG1 \<and>
+         (v, v') \<in> inhst SG1"
+        by (simp add: srcst_def relcomp_unfold)
+      then show "(e, v) \<in> srcst (SG1 USG SG2)"
+      proof
+        fix v'
+        assume h: "(e, v') \<in> EsC SG1 \<lhd> srcr SG1 \<and> (v, v') \<in> inhst SG1"
+        hence "e \<in> EsC SG1" by (simp add: dres_def)
+        hence "e \<in> EsC SG1 \<union> EsC SG2" by auto
+        hence "e \<in> EsC (SG1 USG SG2)" 
+          using assms by (simp add: EsC_USG)
+        from h have "(e, v') \<in> srcr SG1" 
+          by (simp add: dres_def)
+        hence "(e, v') \<in> srcr (SG1 USG SG2)"
+          using assms by (simp add: srcr_USG)
+        from h have "(v, v') \<in> inhst SG1" by auto
+        hence "(v, v') \<in> inhst (SG1 USG SG2)"
+          using assms by (simp add: inhst_USG)
+        then show "(e, v) \<in> srcst (SG1 USG SG2)"
+          using \<open>e \<in> EsC (SG1 USG SG2)\<close> 
+            \<open>(e, v') \<in> srcr (SG1 USG SG2)\<close>
+          using assms 
+          by (auto simp add: srcst_def dres_def)
+      qed
+    next
+      assume "(e, v) \<in> srcst SG2"
+      hence "\<exists> v'. (e, v') \<in> EsC SG2 \<lhd> srcr SG2 \<and>
+         (v, v') \<in> inhst SG2"
+        by (simp add: srcst_def relcomp_unfold)
+      then show "(e, v) \<in> srcst (SG1 USG SG2)"
+      proof
+        fix v'
+        assume h: "(e, v') \<in> EsC SG2 \<lhd> srcr SG2 \<and> (v, v') \<in> inhst SG2"
+        hence "e \<in> EsC SG2" by (simp add: dres_def)
+        hence "e \<in> EsC SG1 \<union> EsC SG2" by auto
+        hence "e \<in> EsC (SG1 USG SG2)" 
+          using assms by (simp add: EsC_USG)
+        from h have "(e, v') \<in> srcr SG2" 
+          by (simp add: dres_def)
+        hence "(e, v') \<in> srcr (SG1 USG SG2)"
+          using assms by (simp add: srcr_USG)
+        from h have "(v, v') \<in> inhst SG2" by auto
+        hence "(v, v') \<in> inhst (SG1 USG SG2)"
+          using assms by (simp add: inhst_USG)
+        then show "(e, v) \<in> srcst (SG1 USG SG2)"
+          using \<open>e \<in> EsC (SG1 USG SG2)\<close> 
+            \<open>(e, v') \<in> srcr (SG1 USG SG2)\<close>
+          using assms 
+          by (auto simp add: srcst_def dres_def)
+      qed
+    qed
+  qed
+qed
+
+lemma tgtst_USG: 
+  assumes "wf_sg SG1" and "wf_sg SG2" and "disjGs SG1 SG2"
+  shows "tgtst (SG1 USG SG2) = tgtst SG1 \<union> tgtst SG2"
+proof
+  show "tgtst (SG1 USG SG2) \<subseteq> tgtst SG1 \<union> tgtst SG2"
+  proof (rule subrelI)
+    fix e v 
+    assume "(e, v) \<in> tgtst (SG1 USG SG2)"
+    hence "\<exists> v'. (e, v') \<in>  EsC (SG1 USG SG2) \<lhd>tgtr (SG1 USG SG2) 
+      \<and> (v, v') \<in> inhst (SG1 USG SG2)" 
+      using assms by (auto simp add: tgtst_def)
+    then show "(e, v) \<in> tgtst SG1 \<union> tgtst SG2"
+    proof 
+      fix v'
+      assume h: "(e, v') \<in> EsC (SG1 USG SG2) \<lhd> tgtr (SG1 USG SG2) \<and>
+         (v, v') \<in> inhst (SG1 USG SG2)"
+      hence "e \<in> EsC SG1 \<or> e \<in> EsC SG2"
+        using assms by (simp add: EsC_USG dres_def)
+      then show "(e, v) \<in> tgtst SG1 \<union> tgtst SG2"
+      proof
+        assume "e \<in> EsC SG1"
+        hence "e \<in> Es SG1" using assms EsC_sub_Es[of SG1] by auto
+        hence "(e, v') \<in> tgtr SG1"
+          using assms h EsC_sub_Es[of SG1] 
+          disjGs_imp_disjEsGs[of SG1 SG2]
+          dom_tgtr_eq_Es[of SG1] dom_tgtr_eq_Es[of SG2]
+          by (auto simp add: tgtr_USG EsC_USG dres_def disjEsGs_def)
+        hence "v' \<in> Ns SG1" 
+          using assms ran_tgtr_sub_Ns[of SG1] by (auto)
+        have "(v, v') \<in> inhst SG1"
+        proof (rule ccontr)
+          assume "(v, v') \<notin>  inhst SG1"
+          then show "False"
+          proof (case_tac "v = v'")
+            assume "v = v'"
+            then show "False" 
+              using \<open>(v, v') \<notin>  inhst SG1\<close>
+            by (auto simp add: inhst_def)
+          next
+            assume "v \<noteq> v'"
+            hence "(v, v') \<in> inhst SG2"
+              using \<open>(v, v') \<notin>  inhst SG1\<close> h assms
+              by (auto simp add: inhst_USG EsC_USG srcr_USG )
+            hence "v' \<in> Range(inh SG2)" 
+              using \<open>v \<noteq> v'\<close>
+              by (simp add: in_trancl_in_Range inhst_def 
+                  rtrancl_eq_or_trancl)
+              then show "False"
+                using assms \<open>v' \<in> Ns SG1\<close> Range_inh[of SG2]
+                by (auto simp add: inhst_def disjGs_def)
+          qed
+        qed 
+        hence "(e, v) \<in> tgtst SG1"
+          using \<open>e \<in> EsC SG1\<close> \<open>(e, v') \<in> tgtr SG1\<close> 
+          by (auto simp add: tgtst_def dres_def)
+        then show "(e, v) \<in> tgtst SG1 \<union> tgtst SG2" 
+           by simp
+      next
+        assume "e \<in> EsC SG2"
+        hence "e \<in> Es SG2" using assms EsC_sub_Es[of SG2] by auto
+        hence "(e, v') \<in> tgtr SG2"
+          using assms h EsC_sub_Es[of SG2] 
+          disjGs_imp_disjEsGs[of SG1 SG2]
+          dom_tgtr_eq_Es[of SG1] dom_tgtr_eq_Es[of SG2]
+          by (auto simp add: tgtr_USG EsC_USG dres_def disjEsGs_def)
+        hence "v' \<in> Ns SG2" 
+          using assms ran_tgtr_sub_Ns[of SG2] by (auto)
+        have "(v, v') \<in> inhst SG2"
+        proof (rule ccontr)
+          assume "(v, v') \<notin>  inhst SG2"
+          then show "False"
+          proof (case_tac "v = v'")
+            assume "v = v'"
+            then show "False" 
+              using \<open>(v, v') \<notin>  inhst SG2\<close>
+            by (auto simp add: inhst_def)
+          next
+            assume "v \<noteq> v'"
+            hence "(v, v') \<in> inhst SG1"
+              using \<open>(v, v') \<notin>  inhst SG2\<close> h assms
+              by (auto simp add: inhst_USG EsC_USG srcr_USG )
+            hence "v' \<in> Range(inh SG1)" 
+              using \<open>v \<noteq> v'\<close>
+              by (simp add: in_trancl_in_Range inhst_def 
+                  rtrancl_eq_or_trancl)
+            then show "False"
+              using assms \<open>v' \<in> Ns SG2\<close> Range_inh[of SG1]
+              by (auto simp add: inhst_def disjGs_def)
+          qed
+        qed 
+        hence "(e, v) \<in> tgtst SG2"
+          using \<open>e \<in> EsC SG2\<close> \<open>(e, v') \<in> tgtr SG2\<close> 
+          by (auto simp add: tgtst_def dres_def)
+        then show "(e, v) \<in> tgtst SG1 \<union> tgtst SG2" 
+          by simp
+      qed
+    qed
+  qed
+next
+  show "tgtst SG1 \<union> tgtst SG2 \<subseteq> tgtst (SG1 USG SG2)"
+  proof (rule subrelI)
+    fix e v
+    assume "(e, v) \<in> tgtst SG1 \<union> tgtst SG2"
+    then show "(e, v) \<in> tgtst (SG1 USG SG2)"
+    proof
+      assume "(e, v) \<in> tgtst SG1"
+      hence "\<exists> v'. (e, v') \<in> EsC SG1 \<lhd> tgtr SG1 \<and>
+         (v, v') \<in> inhst SG1"
+        by (simp add: tgtst_def relcomp_unfold)
+      then show "(e, v) \<in> tgtst (SG1 USG SG2)"
+      proof
+        fix v'
+        assume h: "(e, v') \<in> EsC SG1 \<lhd> tgtr SG1 \<and> (v, v') \<in> inhst SG1"
+        hence "e \<in> EsC SG1" by (simp add: dres_def)
+        hence "e \<in> EsC SG1 \<union> EsC SG2" by auto
+        hence "e \<in> EsC (SG1 USG SG2)" 
+          using assms by (simp add: EsC_USG)
+        from h have "(e, v') \<in> tgtr SG1" 
+          by (simp add: dres_def)
+        hence "(e, v') \<in> tgtr (SG1 USG SG2)"
+          using assms by (simp add: tgtr_USG)
+        from h have "(v, v') \<in> inhst SG1" by auto
+        hence "(v, v') \<in> inhst (SG1 USG SG2)"
+          using assms by (simp add: inhst_USG)
+        then show "(e, v) \<in> tgtst (SG1 USG SG2)"
+          using \<open>e \<in> EsC (SG1 USG SG2)\<close> 
+            \<open>(e, v') \<in> tgtr (SG1 USG SG2)\<close>
+          using assms 
+          by (auto simp add: tgtst_def dres_def)
+      qed
+    next
+      assume "(e, v) \<in> tgtst SG2"
+      hence "\<exists> v'. (e, v') \<in> EsC SG2 \<lhd> tgtr SG2 \<and>
+         (v, v') \<in> inhst SG2"
+        by (simp add: tgtst_def relcomp_unfold)
+      then show "(e, v) \<in> tgtst (SG1 USG SG2)"
+      proof
+        fix v'
+        assume h: "(e, v') \<in> EsC SG2 \<lhd> tgtr SG2 \<and> (v, v') \<in> inhst SG2"
+        hence "e \<in> EsC SG2" by (simp add: dres_def)
+        hence "e \<in> EsC SG1 \<union> EsC SG2" by auto
+        hence "e \<in> EsC (SG1 USG SG2)" 
+          using assms by (simp add: EsC_USG)
+        from h have "(e, v') \<in> tgtr SG2" 
+          by (simp add: dres_def)
+        hence "(e, v') \<in> tgtr (SG1 USG SG2)"
+          using assms by (simp add: tgtr_USG)
+        from h have "(v, v') \<in> inhst SG2" by auto
+        hence "(v, v') \<in> inhst (SG1 USG SG2)"
+          using assms by (simp add: inhst_USG)
+        then show "(e, v) \<in> tgtst (SG1 USG SG2)"
+          using \<open>e \<in> EsC (SG1 USG SG2)\<close> 
+            \<open>(e, v') \<in> tgtr (SG1 USG SG2)\<close>
+          using assms 
+          by (auto simp add: tgtst_def dres_def)
+      qed
+    qed
+  qed
+qed
+    
+lemma EsIncidentst_USG:
+  assumes "wf_sg SG1" and "wf_sg SG2" and "disjGs SG1 SG2"
+  shows "(SG1 USG SG2) \<circ>\<rightarrow>\<circ>\<^sup>* vs = SG1 \<circ>\<rightarrow>\<circ>\<^sup>* vs \<union> SG2 \<circ>\<rightarrow>\<circ>\<^sup>* vs"
+  using assms
+  by (auto simp add: esIncidentst_def srcst_USG tgtst_USG)
+
+lemma EsIncidentst_Un_disj_vs:
+  assumes "wf_sg SG" and "vs2 \<inter> Ns SG = {}" 
+  shows "SG \<circ>\<rightarrow>\<circ>\<^sup>* (vs1 \<union> vs2) = SG \<circ>\<rightarrow>\<circ>\<^sup>* vs1"
+  using assms 
+  by (simp add: esIncidentst_Un esIncidentst_disjoint_vs)
 (*lemma EsI_disj_dist: "\<lbrakk>is_wf_sg SG1; is_wf_sg SG2; disjGs SG1 SG2\<rbrakk>
   \<Longrightarrow>EsI (SG1 USG SG2) = EsI SG1 \<union> EsI SG2"
 proof -
@@ -1161,284 +1431,27 @@ qed*)
   qed
 qed*)
 
-lemma restrict_cup_wf_1: 
-  assumes "wf_sg SG1" and "wf_sg SG2" and "disjGs SG1 SG2"
-  shows "SG1 \<bowtie>\<^sub>E\<^sub>S (EsI SG1 \<union> EsI SG2) = SG1 \<bowtie>\<^sub>E\<^sub>S EsI SG1"
-proof -
-  have "EsI SG2 \<inter> Es SG1 = {}"
-    using assms(2) assms(3) EsI_sub_Es[of SG2]
-    by (auto simp add: disjGs_def disjEsGs_def)
-  then show ?thesis
-    using assms wf_sg_wf_g[of SG1] wf_sg_wf_g[of SG2]
-    by (simp add: restrict_dist_cup_es)
-qed
 
-lemma disjGs_inhG:
-  assumes "wf_sg SG1" and "wf_sg SG2" and "disjGs SG1 SG2"
-  shows "disjGs (inhG SG1) (inhG SG2)"
-proof (simp add: disjGs_def)
-  apply_end(rule conjI)
-  show "rst_Ns SG1 (EsI SG1) \<inter> rst_Ns SG2 (EsI SG2) = {}"
-    using assms wf_sg_wf_g[of SG1] wf_sg_wf_g[of SG2]
-      ran_src_G[of SG1] ran_src_G[of SG2] 
-      ran_tgt_G[of SG1] ran_tgt_G[of SG2] 
-      ran_restrict_sub[of "src SG1" "EsI SG1"]
-      ran_restrict_sub[of "src SG2" "EsI SG2"]
-      ran_restrict_sub[of "tgt SG1" "EsI SG1"]
-      ran_restrict_sub[of "tgt SG2" "EsI SG2"]
-    unfolding rst_Ns_def disjGs_def by force
-next
-  apply_end(rule conjI)
-  show "rst_Ns SG1 (EsI SG1) \<inter> (Es SG1 \<inter> EsI SG1) = {}"
-    using assms(1) assms(3) disj_V_E wf_sg_wf_g[of SG1]
-      ran_restrict_sub[of "src SG1" "EsI SG1"]
-      ran_restrict_sub[of "tgt SG1" "EsI SG1"]
-    by (auto simp add: rst_Ns_def wf_g_def disjGs_def 
-        ftotal_on_def)
-next
-  apply_end(rule conjI)
-  show "rst_Ns SG1 (EsI SG1) \<inter> (Es SG2 \<inter> EsI SG2) = {}"
-    using assms(1) assms(3) disj_V_E wf_sg_wf_g[of SG1]
-      ran_restrict_sub[of "src SG1" "EsI SG1"]
-      ran_restrict_sub[of "tgt SG1" "EsI SG1"]
-    by (auto simp add: rst_Ns_def wf_g_def disjGs_def 
-        ftotal_on_def)
-next
-  apply_end(rule conjI)
-  show "rst_Ns SG2 (EsI SG2) \<inter> (Es SG1 \<inter> EsI SG1) = {}"
-    using assms(2) assms(3) disj_V_E wf_sg_wf_g[of SG2]
-      ran_restrict_sub[of "src SG2" "EsI SG2"]
-      ran_restrict_sub[of "tgt SG2" "EsI SG2"]
-    by (auto simp add: rst_Ns_def wf_g_def disjGs_def 
-        ftotal_on_def)
-next
-  apply_end(rule conjI)
-  show "rst_Ns SG2 (EsI SG2) \<inter> (Es SG2 \<inter> EsI SG2) = {}"
-    using assms(2) assms(3) disj_V_E wf_sg_wf_g[of SG2]
-      ran_restrict_sub[of "src SG2" "EsI SG2"]
-      ran_restrict_sub[of "tgt SG2" "EsI SG2"]
-    by (auto simp add: rst_Ns_def wf_g_def disjGs_def 
-        ftotal_on_def)
-next
-  show "Es SG1 \<inter> EsI SG1 \<inter> (Es SG2 \<inter> EsI SG2) = {}"
-    using assms EsI_sub_Es[of SG1] EsI_sub_Es[of SG2]
-    disjGs_imp_disjEsGs[of SG1 SG2]
-    by (auto simp add:  disjEsGs_def)
-qed
 
-lemma inh_disj_SGs_disj_fields: 
-  assumes "wf_sg SG1" and "wf_sg SG2" and h3: "disjGs SG1 SG2"
-  shows "Field (inh SG1) \<inter> Field (inh SG2) = {}"
-  using assms disjGs_inhG[of SG1 SG2] wf_sg_wf_g[of SG1]
-        wf_sg_wf_g[of SG2] wf_g_inhG[of SG1] wf_g_inhG[of SG2] 
-        by (simp add: inh_def relG_disj_Gs)
-      thm restrict_cup_wf_1
-
-lemma inhG_USG:
-  assumes "wf_sg SG1" and "wf_sg SG2" and "disjGs SG1 SG2"
-  shows "inhG (SG1 USG SG2) = inhG (SG1) UG  inhG (SG2)"
-proof -
-  have h: "EsI SG1 \<union> EsI SG2 = EsI SG2 \<union> EsI SG1" by auto
-  show ?thesis
-  using assms disjGs_imp_disjEsGs[of SG1 SG2]
-    restrict_cup_wf_1[of SG2 SG1] restrict_cup_wf_1[of SG1 SG2]
-  by (simp add: inhG_def restrict_USG EsI_USG 
-      disjGs_sym h)
-qed
-
-lemma inh_USG:
-  assumes "wf_sg SG1" and "wf_sg SG2" and "disjGs SG1 SG2"
-  shows "inh (SG1 USG SG2) = inh (SG1) \<union>  inh (SG2)"
-proof -
-  have h1: "EsI SG1 \<union> EsI SG2 = EsI SG2 \<union> EsI SG1" by auto
-  have h2: "SG1 \<bowtie>\<^sub>E\<^sub>S EsI SG1 = inhG SG1" 
-    by (simp add: inhG_def)
-  have h3: "SG2 \<bowtie>\<^sub>E\<^sub>S EsI SG2 = inhG SG2" 
-    by (simp add: inhG_def)
-  show ?thesis
-  using assms disjGs_imp_disjEsGs[of SG1 SG2]
-      wf_sg_wf_g[of SG1] wf_sg_wf_g[of SG2]
-      disjGs_inhG[of SG1 SG2] wf_g_inhG[of SG1] wf_g_inhG[of SG2]
-      disjGs_imp_disjEsGs[of "inhG SG1" "inhG SG2"]
-      restrict_cup_wf_1[of SG2 SG1] restrict_cup_wf_1[of SG1 SG2]
-  by (simp add: inh_def inhG_def restrict_USG EsI_USG 
-      disjGs_sym h1, (subst h2)+, (subst h3)+)
-      (simp add: relG_UG)
-qed
 
 lemma srcma_disj_SGs:
   assumes "wf_sg SG1" and "wf_sg SG2" and "disjGs SG1 SG2"
   shows "dom(srcma SG1) \<inter> dom(srcma SG2) = {}"
   using assms wf_sg_ftotal_on_srcma[of SG1]
         wf_sg_ftotal_on_srcma[of SG2] 
-        disjGs_imp_disjEsGs[of SG1 SG2] EsC_sub_ES[of SG1]
-        EsC_sub_ES[of SG2]
+        disjGs_imp_disjEsGs[of SG1 SG2] EsC_sub_Es[of SG1]
+        EsC_sub_Es[of SG2]
       by (simp add: ftotal_on_def disjEsGs_def, force)
 
-lemma dom_srcma_ecomp_uni_sub_dom_srcma:
-  shows "dom(srcma_ecomp_uni SG) \<subseteq> dom(srcma SG)"
-  by (simp add: srcma_def subsetI)
-
-lemma dom_srcma_erel_uni_sub_dom_srcma:
-  shows "dom(srcma_erel_uni SG) \<subseteq> dom(srcma SG)"
-  by (simp add: srcma_def subsetI)
-
-lemma srcma_ecomp_uni_USG_in_SG1:
-  assumes "wf_sg SG1" and "wf_sg SG2" and "disjGs SG1 SG2"
-    and "e \<in> Es SG1"
-  shows "srcma_ecomp_uni (SG1 USG SG2) e = srcma_ecomp_uni SG1 e"
-  using assms EsTy_sub_Es[of SG1 "{ecomp duni}"]
-    EsTy_sub_Es[of SG2 "{ecomp duni}"]
-    disjGs_imp_disjEsGs[of "SG1" "SG2"]
-  by (auto simp add: srcma_ecomp_uni_def EsTy_USG disjEsGs_def)
-
-lemma srcma_ecomp_uni_USG_nin_SG1:
-  assumes "wf_sg SG1" and "wf_sg SG2" and "disjGs SG1 SG2"
-    and "e \<notin> Es SG1"
-  shows "srcma_ecomp_uni (SG1 USG SG2) e = srcma_ecomp_uni SG2 e"
-  using assms EsTy_sub_Es[of SG1 "{ecomp duni}"]
-          EsTy_sub_Es[of SG2 "{ecomp duni}"]
-          disjGs_imp_disjEsGs[of "SG1" "SG2"]
-  by (auto simp add: srcma_ecomp_uni_def EsTy_USG disjEsGs_def)
-  
-lemma srcma_ecomp_uni_USG:
-  assumes "wf_sg SG1" and "wf_sg SG2" and "disjGs SG1 SG2"
-  shows "srcma_ecomp_uni (SG1 USG SG2) = (srcma_ecomp_uni SG1) ++ (srcma_ecomp_uni SG2)"
-proof -
-  have h: "dom(srcma_ecomp_uni SG1) \<inter> dom(srcma_ecomp_uni SG2) = {}"
-    using assms dom_srcma_ecomp_uni_sub_dom_srcma[of SG1]
-      dom_srcma_ecomp_uni_sub_dom_srcma[of SG2]
-      srcma_disj_SGs[of SG1 SG2]
-    by (auto)
-  show ?thesis
-  proof
-    fix e
-    show "srcma_ecomp_uni (SG1 USG SG2) e =
-         (srcma_ecomp_uni SG1 ++ srcma_ecomp_uni SG2) e"
-    proof (case_tac "e \<in> Es SG1")
-      assume h1: "e \<in> Es SG1"
-      hence h2: "srcma_ecomp_uni (SG1 USG SG2) e = srcma_ecomp_uni SG1 e"
-        using assms by (simp add: srcma_ecomp_uni_USG_in_SG1)
-      have "e \<notin> dom(srcma_ecomp_uni SG2)"
-      proof (rule ccontr, simp)
-        assume "e \<in> dom (srcma_ecomp_uni SG2)"
-        then show "False" 
-          using EsC_sub_ES assms(2) assms(3) disjGs_imp_disjEsGs 
-              es_disj_Ga_Gb ftotal_on_dom h1 srcma_def 
-              wf_sg_ftotal_on_srcma by fastforce
-      qed
-      hence "(srcma_ecomp_uni SG1 ++ srcma_ecomp_uni SG2) e = srcma_ecomp_uni SG1 e"
-        using h map_add_disj_dom2f[where f = "srcma_ecomp_uni SG1"]
-        by simp
-      then show "srcma_ecomp_uni (SG1 USG SG2) e =
-        (srcma_ecomp_uni SG1 ++ srcma_ecomp_uni SG2) e"
-        using h2 by auto
-    next
-      assume h1: "e \<notin> Es SG1"
-      hence h2: "srcma_ecomp_uni (SG1 USG SG2) e = srcma_ecomp_uni SG2 e"
-        using assms by (simp add: srcma_ecomp_uni_USG_nin_SG1)
-      have "e \<notin> dom(srcma_ecomp_uni SG1)"
-      proof (rule ccontr, simp)
-        assume "e \<in> dom (srcma_ecomp_uni SG1)"
-        then show "False" 
-          using EsC_sub_ES assms(1) assms(3) disjGs_imp_disjEsGs 
-              es_disj_Ga_Gb ftotal_on_dom h1 srcma_def 
-              wf_sg_ftotal_on_srcma by fastforce
-      qed
-      hence "(srcma_ecomp_uni SG1 ++ srcma_ecomp_uni SG2) e = srcma_ecomp_uni SG2 e"
-        using h map_add_disj_dom2f[where x = e and f = "srcma_ecomp_uni SG2" and g = "srcma_ecomp_uni SG1"]
-        map_add_comm[of "srcma_ecomp_uni SG1" "srcma_ecomp_uni SG2"]
-        by force
-      then show "srcma_ecomp_uni (SG1 USG SG2) e =
-        (srcma_ecomp_uni SG1 ++ srcma_ecomp_uni SG2) e"
-        using h2 by auto
-    qed
-  qed
-qed
-
-lemma srcma_erel_uni_USG_in_SG1:
-  assumes "wf_sg SG1" and "wf_sg SG2" and "disjGs SG1 SG2"
-    and "e \<in> Es SG1"
-  shows "srcma_erel_uni (SG1 USG SG2) e = srcma_erel_uni SG1 e"
-  using assms EsTy_sub_Es[of SG1 "{erel duni}"]
-    EsTy_sub_Es[of SG2 "{erel duni}"]
-    disjGs_imp_disjEsGs[of "SG1" "SG2"]
-  by (auto simp add: srcma_erel_uni_def EsTy_USG disjEsGs_def)
-
-lemma srcma_erel_uni_USG_nin_SG1:
-  assumes "wf_sg SG1" and "wf_sg SG2" and "disjGs SG1 SG2"
-    and "e \<notin> Es SG1"
-  shows "srcma_erel_uni (SG1 USG SG2) e = srcma_erel_uni SG2 e"
-  using assms EsTy_sub_Es[of SG1 "{erel duni}"]
-          EsTy_sub_Es[of SG2 "{erel duni}"]
-          disjGs_imp_disjEsGs[of "SG1" "SG2"]
-  by (auto simp add: srcma_erel_uni_def EsTy_USG disjEsGs_def)
-
-lemma srcma_erel_uni_USG:
-  assumes "wf_sg SG1" and "wf_sg SG2" and "disjGs SG1 SG2"
-  shows "srcma_erel_uni (SG1 USG SG2) = (srcma_erel_uni SG1) ++ (srcma_erel_uni SG2)"
-proof -
-  have h: "dom(srcma_erel_uni SG1) \<inter> dom(srcma_erel_uni SG2) = {}"
-  using assms dom_srcma_erel_uni_sub_dom_srcma[of SG1]
-      dom_srcma_erel_uni_sub_dom_srcma[of SG2]
-      srcma_disj_SGs[of SG1 SG2]
-    by (auto)
-  show ?thesis
-  proof
-    fix e
-    show "srcma_erel_uni (SG1 USG SG2) e =
-         (srcma_erel_uni SG1 ++ srcma_erel_uni SG2) e"
-    proof (case_tac "e \<in> Es SG1")
-      assume h1: "e \<in> Es SG1"
-      hence h2: "srcma_erel_uni (SG1 USG SG2) e = srcma_erel_uni SG1 e"
-        using assms srcma_erel_uni_USG_in_SG1 by auto
-      have "e \<notin> dom(srcma_erel_uni SG2)"
-      proof (rule ccontr, simp)
-        assume "e \<in> dom (srcma_erel_uni SG2)"
-        then show "False" 
-          using EsC_sub_ES assms(2) assms(3) disjGs_imp_disjEsGs 
-              es_disj_Ga_Gb ftotal_on_dom h1 srcma_def 
-              wf_sg_ftotal_on_srcma by fastforce
-      qed
-      hence "(srcma_erel_uni SG1 ++ srcma_erel_uni SG2) e = srcma_erel_uni SG1 e"
-        using h map_add_disj_dom2f[where f = "srcma_erel_uni SG1"]
-        by simp
-      then show "srcma_erel_uni (SG1 USG SG2) e =
-        (srcma_erel_uni SG1 ++ srcma_erel_uni SG2) e"
-        using h2 by auto
-    next
-      assume h1: "e \<notin> Es SG1"
-      hence h2: "srcma_erel_uni (SG1 USG SG2) e = srcma_erel_uni SG2 e"
-        using assms srcma_erel_uni_USG_nin_SG1 by auto
-      have "e \<notin> dom(srcma_erel_uni SG1)"
-      proof (rule ccontr, simp)
-        assume "e \<in> dom (srcma_erel_uni SG1)"
-        then show "False" 
-          using EsC_sub_ES assms(1) assms(3) disjGs_imp_disjEsGs 
-              es_disj_Ga_Gb ftotal_on_dom h1 srcma_def 
-              wf_sg_ftotal_on_srcma by fastforce
-      qed
-      hence "(srcma_erel_uni SG1 ++ srcma_erel_uni SG2) e = srcma_erel_uni SG2 e"
-        using h map_add_disj_dom2f[where x = e and f = "srcma_erel_uni SG2" and g = "srcma_erel_uni SG1"]
-        map_add_comm[of "srcma_erel_uni SG1" "srcma_erel_uni SG2"]
-        by force
-      then show "srcma_erel_uni (SG1 USG SG2) e =
-        (srcma_erel_uni SG1 ++ srcma_erel_uni SG2) e"
-        using h2 by auto
-    qed
-  qed
-qed
- 
 lemma srcma_USG:
   assumes "wf_sg SG1" and "wf_sg SG2" and "disjGs SG1 SG2"
   shows "srcma (SG1 USG SG2) = srcma (SG1) ++ srcma (SG2)"
 proof
   fix e
   show "srcma (SG1 USG SG2) e = (srcma (SG1) ++ srcma (SG2)) e"
-    by (smt (verit, ccfv_threshold) assms disjoint_iff domIff 
+    by (smt (z3) EsTy_USG Un_iff assms disjoint_iff domIff 
         map_add_dom_app_simps(1) map_add_dom_app_simps(3) 
-        srcm_cupSG srcma_def srcma_disj_SGs 
-        srcma_ecomp_uni_USG srcma_erel_uni_USG)
+        srcm_cupSG srcma_def srcma_disj_SGs)  
 qed
 
 lemma acyclic_SGr_Un_dist: 
@@ -1450,6 +1463,236 @@ lemma acyclic_SGr_Un_dist:
     disjGs_inhG[of SG1 SG2]
   by (simp add: inhG_USG acyclic_Gr_dist_disj)
 
+lemma multsOk_USG:
+  assumes "wf_sg SG1" and "wf_sg SG2" and "disjGs SG1 SG2"
+  shows "multsOk (SG1 USG SG2)"
+  by (smt (z3) EsC_USG EsC_sub_Es SGr.select_convs(2) Un_iff 
+      assms cupSG_def disjGs_imp_disjEsGs es_disj_Ga_Gb 
+      ftotal_on_dom map_add_disj_domf map_add_dom_app_simps(1) 
+      multsOk_def srcma_USG srcma_disj_SGs subset_Un_eq 
+      tgtm_cupSG wf_sg_def)
+
+  
+lemma optsVoluntary_USG:
+  assumes "wf_sg SG1" and "wf_sg SG2" and "disjGs SG1 SG2"
+  shows "optsVoluntary (SG1 USG SG2)"
+proof -
+  have h1: "optsVoluntary SG1" using assms(1) by (simp add: wf_sg_def)
+  have h2: "optsVoluntary SG2" using assms(2) by (simp add: wf_sg_def)
+  have h3: "NsO SG2 \<inter> Ns SG1 = {}" using assms NsO_sub_Ns[of SG2]
+    by (auto simp add: disjGs_def)
+  have h4: "NsO SG1 \<inter> Ns SG2 = {}" using assms NsO_sub_Ns[of SG1]
+    by (auto simp add: disjGs_def)
+  have h5: "(SG1 \<circ>\<rightarrow>\<circ>\<^sup>* NsO SG1 \<union> SG2 \<circ>\<rightarrow>\<circ>\<^sup>* NsO SG2 - (EsI SG1 \<union> EsI SG2))
+    = (SG1 \<circ>\<rightarrow>\<circ>\<^sup>* NsO SG1) - EsI SG1 \<union> (SG2 \<circ>\<rightarrow>\<circ>\<^sup>* NsO SG2) - EsI SG2"
+    using assms EsI_sub_Es[of SG1] EsI_sub_Es[of SG2]
+    disjGs_imp_disjEsGs[of SG1 SG2]
+    esIncidentst_SG_Sub_EsSG[of SG1 "NsO SG1"]
+    esIncidentst_SG_Sub_EsSG[of SG2 "NsO SG2"]
+    by (auto simp add: disjEsGs_def)
+  have h6: "dom (ety SG1) \<inter> dom (ety SG2) = {}" 
+    using assms disjGs_imp_disjEsGs[of SG1 SG2] 
+    wf_sg_ftotal_on_ety[of SG1] wf_sg_ftotal_on_ety[of SG2]
+    by (simp add: disjEsGs_def ftotal_on_def)
+  have h7: "(SG1 \<circ>\<rightarrow>\<circ>\<^sup>* NsO SG1 - EsI SG1) \<inter> Es SG2 = {}"
+    using assms(1) assms(3) disjGs_imp_disjEsGs 
+      esIncidentst_SG_Sub_EsSG es_disj_Ga_Gb 
+    by fastforce
+  have h8: "(SG2 \<circ>\<rightarrow>\<circ>\<^sup>* NsO SG2 - EsI SG2) \<inter> Es SG1 = {}"
+    using assms(2) assms(3) disjGs_imp_disjEsGs 
+      esIncidentst_SG_Sub_EsSG es_disj_Ga_Gb 
+    by fastforce
+  have h9: "(pfunToRel (ety SG1) \<union> pfunToRel (ety SG2)) ``
+    (SG1 \<circ>\<rightarrow>\<circ>\<^sup>* NsO SG1 - EsI SG1 \<union> SG2 \<circ>\<rightarrow>\<circ>\<^sup>* NsO SG2 - EsI SG2)
+    =  pfunToRel (ety SG1) `` (SG1 \<circ>\<rightarrow>\<circ>\<^sup>* NsO SG1 - EsI SG1)
+    \<union> pfunToRel (ety SG2) `` (SG2 \<circ>\<rightarrow>\<circ>\<^sup>* NsO SG2 - EsI SG2)"
+  proof
+    show "(pfunToRel (ety SG1) \<union> pfunToRel (ety SG2)) ``
+    (SG1 \<circ>\<rightarrow>\<circ>\<^sup>* NsO SG1 - EsI SG1 \<union> SG2 \<circ>\<rightarrow>\<circ>\<^sup>* NsO SG2 - EsI SG2)
+    \<subseteq> pfunToRel (ety SG1) `` (SG1 \<circ>\<rightarrow>\<circ>\<^sup>* NsO SG1 - EsI SG1) \<union>
+       pfunToRel (ety SG2) `` (SG2 \<circ>\<rightarrow>\<circ>\<^sup>* NsO SG2 - EsI SG2)"
+    proof
+      fix x
+      assume "x \<in> (pfunToRel (ety SG1) \<union> pfunToRel (ety SG2)) ``
+             (SG1 \<circ>\<rightarrow>\<circ>\<^sup>* NsO SG1 - EsI SG1 \<union> SG2 \<circ>\<rightarrow>\<circ>\<^sup>* NsO SG2 -
+              EsI SG2)"
+      hence "x \<in> (pfunToRel (ety SG1) \<union> pfunToRel (ety SG2)) `` 
+          (SG1 \<circ>\<rightarrow>\<circ>\<^sup>* NsO SG1 - EsI SG1) 
+          \<union> (pfunToRel (ety SG1) \<union> pfunToRel (ety SG2)) `` (SG2 \<circ>\<rightarrow>\<circ>\<^sup>* NsO SG2 -
+              EsI SG2)" by auto
+      hence "x \<in> pfunToRel (ety SG1) `` (SG1 \<circ>\<rightarrow>\<circ>\<^sup>* NsO SG1 - EsI SG1)
+        \<union> pfunToRel (ety SG1) `` (SG2 \<circ>\<rightarrow>\<circ>\<^sup>* NsO SG2 - EsI SG2)
+        \<union> pfunToRel (ety SG2) `` (SG1 \<circ>\<rightarrow>\<circ>\<^sup>* NsO SG1 - EsI SG1)
+        \<union> pfunToRel (ety SG2) `` (SG2 \<circ>\<rightarrow>\<circ>\<^sup>* NsO SG2 - EsI SG2)" 
+        by auto  
+      then show "x \<in> pfunToRel (ety SG1) `` (SG1 \<circ>\<rightarrow>\<circ>\<^sup>* NsO SG1 - EsI SG1) \<union>
+              pfunToRel (ety SG2) `` (SG2 \<circ>\<rightarrow>\<circ>\<^sup>* NsO SG2 - EsI SG2)"
+       using h7 h8 assms wf_sg_ftotal_on_ety[of SG1] 
+            wf_sg_ftotal_on_ety[of SG2]
+        by (simp add: Image_outside_domain ftotal_on_def
+            disjGs_imp_disjEsGs es_disj_Ga_Gb Domain_is_dom)
+    qed
+  next
+    show "pfunToRel (ety SG1) `` (SG1 \<circ>\<rightarrow>\<circ>\<^sup>* NsO SG1 - EsI SG1) \<union>
+    pfunToRel (ety SG2) `` (SG2 \<circ>\<rightarrow>\<circ>\<^sup>* NsO SG2 - EsI SG2)
+    \<subseteq> (pfunToRel (ety SG1) \<union> pfunToRel (ety SG2)) ``
+       (SG1 \<circ>\<rightarrow>\<circ>\<^sup>* NsO SG1 - EsI SG1 \<union> SG2 \<circ>\<rightarrow>\<circ>\<^sup>* NsO SG2 - EsI SG2)"
+    proof
+      fix x
+      assume "x \<in> pfunToRel (ety SG1) `` (SG1 \<circ>\<rightarrow>\<circ>\<^sup>* NsO SG1 - EsI SG1) \<union>
+      pfunToRel (ety SG2) `` (SG2 \<circ>\<rightarrow>\<circ>\<^sup>* NsO SG2 - EsI SG2)"
+      then show "x \<in> (pfunToRel (ety SG1) \<union> pfunToRel (ety SG2)) ``
+              (SG1 \<circ>\<rightarrow>\<circ>\<^sup>* NsO SG1 - EsI SG1 \<union> SG2 \<circ>\<rightarrow>\<circ>\<^sup>* NsO SG2 -
+               EsI SG2)" 
+      proof
+        assume "x \<in> pfunToRel (ety SG1) `` (SG1 \<circ>\<rightarrow>\<circ>\<^sup>* NsO SG1 - EsI SG1)"
+        hence "x \<in> (pfunToRel (ety SG1) \<union> pfunToRel (ety SG2)) `` 
+          (SG1 \<circ>\<rightarrow>\<circ>\<^sup>* NsO SG1 - EsI SG1)"
+          by auto
+        then show "x \<in> (pfunToRel (ety SG1) \<union> pfunToRel (ety SG2)) ``
+              (SG1 \<circ>\<rightarrow>\<circ>\<^sup>* NsO SG1 - EsI SG1 \<union> SG2 \<circ>\<rightarrow>\<circ>\<^sup>* NsO SG2 - EsI SG2)"
+          by (smt (verit, ccfv_SIG) DiffI EsI_sub_Es ImageE ImageI IntD1 Un_Int_eq(1) assms(2) disjoint_iff h7 subset_eq)
+      next
+        assume "x \<in> pfunToRel (ety SG2) `` (SG2 \<circ>\<rightarrow>\<circ>\<^sup>* NsO SG2 - EsI SG2)"
+        then show "x \<in> (pfunToRel (ety SG1) \<union> pfunToRel (ety SG2)) ``
+              (SG1 \<circ>\<rightarrow>\<circ>\<^sup>* NsO SG1 - EsI SG1 \<union> SG2 \<circ>\<rightarrow>\<circ>\<^sup>* NsO SG2 - EsI SG2)"
+         by auto
+      qed
+    qed
+  qed
+  show ?thesis
+    using assms h1 h2 h3 h4
+    esIncidentst_disjoint_vs[of SG1 "NsO SG2"]
+    esIncidentst_disjoint_vs[of SG2 "NsO SG1"]
+    wf_sg_ftotal_on_ety[of SG1] wf_sg_ftotal_on_ety[of SG2]
+    h6 
+  by (simp add: optsVoluntary_def NsO_USG EsI_USG 
+      EsIncidentst_USG wf_sg_def esIncidentst_Un h5
+      ftotal_on_def pfunToRel_map_add h9)
+qed
+
+lemma inhOk_SG1_USG_SG2:
+  assumes "wf_sg SG1" and "wf_sg SG2" and "disjGs SG1 SG2"
+  shows "inhOk (SG1 USG SG2)"
+proof-
+  have h1: "acyclicGr (inhG SG1)" 
+    using assms(1) by (simp add: wf_sg_def inhOk_def)
+  have h2: "acyclicGr (inhG SG2)" 
+    using assms(2) by (simp add: wf_sg_def inhOk_def)
+  have h3: "pfun_on ((inhG SG1  \<ominus>\<^sub>N\<^sub>S NsV SG1 )\<^sup>\<Leftrightarrow>) (Ns (SG1)) (Ns (SG1))"
+    using assms(1) by (simp add: wf_sg_def inhOk_def)
+  have h4: "pfun_on ((inhG SG2  \<ominus>\<^sub>N\<^sub>S NsV SG2 )\<^sup>\<Leftrightarrow>) (Ns (SG2)) (Ns (SG2))"
+    using assms(2) by (simp add: wf_sg_def inhOk_def)
+  show ?thesis
+  proof (simp add: inhOk_def)
+    apply_end (rule conjI)
+    show "\<forall>v v'.
+       (v, v') \<in> inh (SG1 USG SG2) \<longrightarrow>
+       the ((nty SG1 ++ nty SG2) v) <\<^sub>N\<^sub>T the ((nty SG1 ++ nty SG2) v')"
+    proof (clarsimp)
+      fix v v'
+      assume "(v, v') \<in> inh (SG1 USG SG2)"
+      hence "(v, v') \<in> (inh SG1) \<or> (v, v') \<in> (inh SG2)"
+        using assms by (simp add: inh_USG)
+      then show "the ((nty SG1 ++ nty SG2) v) <\<^sub>N\<^sub>T the ((nty SG1 ++ nty SG2) v')"
+      proof
+        assume "(v, v') \<in> inh SG1"
+        hence "v \<in> Ns SG1" 
+          using assms(1) Domain_inh 
+          by (auto simp add: Domain_iff)
+        hence ha: "(nty SG1 ++ nty SG2) v = nty SG1 v"
+          using assms wf_sg_ftotal_on_nty[of SG1]
+            wf_sg_ftotal_on_nty[of SG2]
+          by (simp add: ftotal_on_dom map_add_disj_domf ns_disj_Ga_Gb)
+        have "v' \<in> Ns SG1"
+          using assms(1) Range_inh \<open>(v, v') \<in> inh SG1\<close>
+          by (auto simp add: Range_iff)
+        hence hb: "(nty SG1 ++ nty SG2) v' = nty SG1 v'"
+          using assms wf_sg_ftotal_on_nty[of SG1]
+            wf_sg_ftotal_on_nty[of SG2]
+          by (simp add: ftotal_on_dom map_add_disj_domf ns_disj_Ga_Gb)
+        show "the ((nty SG1 ++ nty SG2) v) <\<^sub>N\<^sub>T the ((nty SG1 ++ nty SG2) v')"
+          using \<open>(v, v') \<in> inh SG1\<close> assms(1) ha hb inhOk_def wf_sg_def 
+          by auto
+      next
+        assume "(v, v') \<in> inh SG2"
+        hence "v \<in> Ns SG2" 
+          using assms(2) Domain_inh 
+          by (auto simp add: Domain_iff)
+        hence ha: "(nty SG1 ++ nty SG2) v = nty SG2 v"
+          using assms wf_sg_ftotal_on_nty[of SG1]
+            wf_sg_ftotal_on_nty[of SG2] 
+            map_add_disj_domf[of "nty SG2" "nty SG1" v]
+          by (auto simp add: ftotal_on_def map_add_comm disjGs_def)
+        have "v' \<in> Ns SG2"
+          using assms(2) Range_inh \<open>(v, v') \<in> inh SG2\<close>
+          by (auto simp add: Range_iff)
+        hence hb: "(nty SG1 ++ nty SG2) v' = nty SG2 v'"
+          using assms wf_sg_ftotal_on_nty[of SG1]
+            wf_sg_ftotal_on_nty[of SG2]
+            map_add_disj_domf[of "nty SG2" "nty SG1" v']
+          by (auto simp add: ftotal_on_dom map_add_disj_domf map_add_comm
+              disjGs_def)
+        show "the ((nty SG1 ++ nty SG2) v) <\<^sub>N\<^sub>T the ((nty SG1 ++ nty SG2) v')"
+          using \<open>(v, v') \<in> inh SG2\<close> assms(2) ha hb inhOk_def wf_sg_def 
+          by auto
+      qed
+    qed
+  next
+    apply_end (rule conjI)
+    show "acyclicGr (inhG (SG1 USG SG2))"
+      using assms h1 h2 by (simp add: acyclic_SGr_Un_dist)
+  next
+    have ha: "NsV SG2 \<inter> Ns (inhG SG1) = {}" 
+      using assms ran_src_G[of SG1] wf_sg_wf_g[of SG1]
+        ran_tgt_G[of SG1]
+        NsV_sub_Ns[of SG2] ns_disj_Ga_Gb 
+      by (metis (no_types, lifting) Ns_inhG disjoint_iff_not_equal 
+          rst_Ns_sub subsetD)
+    have hb: "NsV SG1  \<inter> Ns (inhG SG2) = {}" 
+      using assms ran_src_G[of SG2] wf_sg_wf_g[of SG2]
+        ran_tgt_G[of SG2]
+        NsV_sub_Ns[of SG1] ns_disj_Ga_Gb 
+      by (metis (no_types, lifting) Ns_inhG disjoint_iff_not_equal 
+          rst_Ns_sub subsetD)
+    have hc: "NsV SG1 \<union> NsV SG2 = NsV SG2 Un NsV SG1" by auto
+    have hd: "inhG SG1 \<ominus>\<^sub>N\<^sub>S (NsV (SG1 USG SG2)) = inhG SG1 \<ominus>\<^sub>N\<^sub>S (NsV SG1)"
+      using assms subtract_Ns_disj[of "inhG SG1" "NsV SG2"] 
+      NsV_sub_Ns[of SG1] NsV_sub_Ns[of SG2] 
+      ns_disj_Ga_Gb[of SG1 SG2] ha wf_g_inhG[of SG1]
+      wf_sg_wf_g[of SG1] 
+      by (simp only: NsV_USG subtract_Ns_disj subtract_Ns_Un hc)
+    have he: "inhG SG2 \<ominus>\<^sub>N\<^sub>S (NsV (SG1 USG SG2)) = inhG SG2 \<ominus>\<^sub>N\<^sub>S (NsV SG2)"
+      using assms subtract_Ns_disj[of "inhG SG1" "NsV SG2"] 
+      NsV_sub_Ns[of SG1] NsV_sub_Ns[of SG2] wf_sg_wf_g[of SG1] 
+      ns_disj_Ga_Gb[of SG1 SG2] hb wf_g_inhG[of SG2]
+      wf_sg_wf_g[of SG2] 
+      by (simp only: NsV_USG subtract_Ns_disj subtract_Ns_Un)
+    have hf: "wf_g (inhG SG1 \<ominus>\<^sub>N\<^sub>S NsV SG1)"
+      using assms wf_sg_wf_g[of SG1] wf_g_inhG[of SG1]
+      by (simp add: wf_subtractNs)
+    have hg: "wf_g (inhG SG2 \<ominus>\<^sub>N\<^sub>S NsV SG2)"
+      using assms wf_sg_wf_g[of SG2] wf_g_inhG[of SG2]
+      by (simp add: wf_subtractNs)
+    have hh: "disjEsGs (inhG SG1 \<ominus>\<^sub>N\<^sub>S NsV SG1) (inhG SG2 \<ominus>\<^sub>N\<^sub>S NsV SG2)"
+      using assms disjGs_imp_disjEsGs[of SG1 SG2] 
+        inhG_disj_Es[of SG1 SG2] disjEsGs_subtractG
+      by (simp)
+    show "pfun_on ((inhG (SG1 USG SG2) \<ominus>\<^sub>N\<^sub>S NsV (SG1 USG SG2))\<^sup>\<Leftrightarrow>) (Ns (SG1) \<union>  Ns(SG2)) (Ns (SG1) \<union> Ns(SG2))"
+      using assms disjGs_imp_disjEsGs[of SG1 SG2]
+      wf_sg_wf_g[of SG1] wf_sg_wf_g[of SG2] inhG_USG
+      wf_g_inhG[of SG1] wf_g_inhG[of SG2] 
+      disjGs_imp_disjEsGs[of "inhG SG1" "inhG SG2"]
+      disjGs_inhG[of SG1 SG2] 
+      subtract_Ns_disj[of "inhG SG1" "Ns (inhG SG2)"]
+      subtract_Ns_disj[of "inhG SG2" "Ns (inhG SG1)"]
+      ns_disj_Ga_Gb ha hb h3 h4
+      by (auto simp add: inhG_USG subtract_Ns_UG  hd he hf hg hh 
+          relG_UG pfun_on_Un disjGs_def)
+  qed
+qed
+  
+
 lemma is_wf_sg_Un: 
   assumes "wf_sg SG1" and "wf_sg SG2" and "disjGs SG1 SG2"
   shows "wf_sg (SG1 USG SG2)"
@@ -1460,14 +1703,14 @@ proof (simp add: wf_sg_def)
     by (simp add: is_wf_g_Un2)
 next
   apply_end(rule conjI)
-  show "ftotal_on (nty (SG1 USG SG2)) (Ns (SG1 USG SG2)) SGNT_set"
+  show "ftotal_on (nty SG1 ++ nty SG2) (Ns SG1 \<union> Ns SG2) SGNT_set"
     using assms wf_sg_ftotal_on_nty[of SG1] wf_sg_ftotal_on_nty[of SG2] 
     ftotal_on_map_add[where f = "nty SG1" and g = "nty SG2" 
       and A="Ns SG1" and C="Ns SG2" and B="SGNT_set" and D="SGNT_set"]
     by (auto simp add: cupSG_def  disjGs_def)
 next
   apply_end(rule conjI)
-  show "ftotal_on (ety (SG1 USG SG2)) (Es (SG1 USG SG2)) SGET_set"
+  show "ftotal_on (ety SG1 ++ ety SG2) (Es (SG1 USG SG2)) SGET_set"
     using assms wf_sg_ftotal_on_ety[of SG1] wf_sg_ftotal_on_ety[of SG2] 
     ftotal_on_map_add[where f = "ety SG1" and g = "ety SG2" 
       and A="Es SG1" and C="Es SG2" and B="SGET_set" and D="SGET_set"] 
@@ -1477,7 +1720,7 @@ next
   show "ftotal_on (srcma (SG1 USG SG2)) (EsC (SG1 USG SG2)) MultC_set"
   using assms wf_sg_ftotal_on_srcma[of SG1] 
         wf_sg_ftotal_on_srcma[of SG2] 
-         EsC_sub_ES[of SG1] EsC_sub_ES[of SG2] 
+         EsC_sub_Es[of SG1] EsC_sub_Es[of SG2] 
          disjGs_imp_disjEsGs[of SG1 SG2]
         ftotal_on_map_add[where f = "srcma SG1" and g = "srcma SG2" 
       and A="EsC SG1" and C="EsC SG2" and B="MultC_set" and D="MultC_set"]
@@ -1487,7 +1730,7 @@ next
   show "ftotal_on (tgtm SG1 ++ tgtm SG2) (EsC (SG1 USG SG2)) MultC_set"
   using assms wf_sg_ftotal_on_tgtm[of SG1] 
         wf_sg_ftotal_on_tgtm[of SG2] 
-        EsC_sub_ES[of SG1] EsC_sub_ES[of SG2] 
+        EsC_sub_Es[of SG1] EsC_sub_Es[of SG2] 
         disjGs_imp_disjEsGs[of SG1 SG2]
         ftotal_on_map_add[where f = "tgtm SG1" and g = "tgtm SG2" 
       and A="EsC SG1" and C="EsC SG2" and B="MultC_set" and D="MultC_set"]
@@ -1498,12 +1741,21 @@ next
   using assms wf_sg_dom_db[of SG1] wf_sg_dom_db[of SG2] 
   by (auto simp add:  EsD_USG)
 next
+  apply_end(rule conjI)
   show "multsOk (SG1 USG SG2)"
+    using assms by (simp only: multsOk_USG)
+next
+  apply_end(rule conjI)
+  show "optsVoluntary (SG1 USG SG2)" 
+    using assms by (simp add: optsVoluntary_USG)
+next
+  show "inhOk (SG1 USG SG2)"
+  using assms by (simp add: inhOk_SG1_USG_SG2)
 qed
         
 definition morphSGr :: "SGr \<Rightarrow> SGr \<Rightarrow> Morph set"
 where
-  "morphSGr SG1 SG2 \<equiv> {r. is_wf_sg SG1 \<and> is_wf_sg SG2
+  "morphSGr SG1 SG2 \<equiv> {r. wf_sg SG1 \<and> wf_sg SG2
       \<and> ftotal_on (fV r) (Ns SG1) (Ns SG2) 
       \<and> ftotal_on (fE r) (Es SG1) (Es SG2)  
       \<and> srcst SG1 O pfunToRel(fV r)  \<subseteq> pfunToRel(fE r) O srcst SG2  
@@ -1512,7 +1764,7 @@ where
 
 definition morphGr2SGr :: "Gr \<Rightarrow> SGr \<Rightarrow> Morph set"
 where
-  "morphGr2SGr G1 SG2 \<equiv> {r. is_wf_g G1 \<and> is_wf_sg SG2
+  "morphGr2SGr G1 SG2 \<equiv> {r. wf_g G1 \<and> wf_sg SG2
       \<and> ftotal_on (fV r) (Ns G1) (Ns SG2) 
       \<and> ftotal_on (fE r) (Es G1) (Es SG2)  
       \<and> pfunToRel((fV r) \<circ>\<^sub>m (src G1)) \<subseteq> pfunToRel(fE r) O srcst SG2  
